SystemF/Contexts.v
@@ -1,7 +1,8 @@
 From Tealeaves Require Import
      Functors.List
      LN.Leaf LN.Atom LN.AtomSet LN.AssocList
-     LN.Multisorted.Operations.
+     LN.Multisorted.Operations
+     LN.Multisorted.Theory.
 
 From Multisorted Require Import
      Classes.DTM.
@@ -10,10 +11,12 @@ From Coq Require Import
      Sorting.Permutation.
 
 From Tealeaves.Examples Require Import
-     SystemF.Language.
+     SystemF.Language
+     SystemF.Rewriting.
 
 Implicit Types (x : atom).
 
+Import SetlikeFunctor.Notations.
 Import List.ListNotations.
 Import LN.AssocList.Notations.
 
@@ -44,10 +47,9 @@ Tactic Notation "bursts" :=
          | H : _ |- _ => burst in H
          end; repeat burst.
 
-(** * Infrastructural lemmas for contexts and well-formedness predicates *)
-(******************************************************************************)
-
-(** ** Reasoning principle for scope (<<scoped>>) *)
+(** * Structural lemmas for <<scoped>> *)
+(** These lemmas are actually independent of System F. They could be
+    incorporated into the locally nameless backend. *)
 (******************************************************************************)
 Section scope_lemmas.
 
@@ -56,7 +58,9 @@ Section scope_lemmas.
     `{DTPreModule (list K) S T (mn_op := Monoid_op_list) (mn_unit := Monoid_unit_list)}
     `{! DTM (list K) T}.
 
-  Theorem perm_scoped : forall (t : S leaf) (X : Type) (γ1 γ2 : alist X) (k : K),
+  (** *** Permutation *)
+  (******************************************************************************)
+  Theorem scoped_perm1 : forall (k : K) (t : S leaf) (X : Type) (γ1 γ2 : alist X),
       Permutation γ1 γ2 ->
       scoped S k t (domset γ1) ->
       scoped S k t (domset γ2).
@@ -64,16 +68,18 @@ Section scope_lemmas.
     introv Hperm. unfold scoped. rewrite (perm_domset); eauto.
   Qed.
 
-  Theorem perm_scoped_iff : forall (t : S leaf) (X : Type) (γ1 γ2 : alist X) (k : K),
+  Theorem scoped_perm : forall (k : K) (t : S leaf) (X : Type) (γ1 γ2 : alist X),
       Permutation γ1 γ2 ->
       scoped S k t (domset γ1) <->
       scoped S k t (domset γ2).
   Proof.
     intros. assert (Permutation γ2 γ1) by now symmetry.
-    split; eauto using perm_scoped.
+    split; eauto using scoped_perm1.
   Qed.
 
-  Lemma weak_scoped_app_l : forall (t : S leaf) (X : Type) (γ1 γ2 : alist X) (k : K),
+  (** *** Weakening *)
+  (******************************************************************************)
+  Lemma scoped_weak_l : forall (k : K) (t : S leaf) (X : Type) (γ1 γ2 : alist X),
       scoped S k t (domset γ1) ->
       scoped S k t (domset (γ1 ++ γ2)).
   Proof.
@@ -81,7 +87,7 @@ Section scope_lemmas.
     autorewrite with tea_rw_dom. fsetdec.
   Qed.
 
-  Lemma weak_scoped_app_r : forall (t : S leaf) (X : Type) (γ1 γ2 : alist X) (k : K),
+  Lemma scoped_weak_r : forall (k : K) (t : S leaf) (X : Type) (γ1 γ2 : alist X),
       scoped S k t (domset γ2) ->
       scoped S k t (domset (γ1 ++ γ2)).
   Proof.
@@ -89,7 +95,9 @@ Section scope_lemmas.
     autorewrite with tea_rw_dom. fsetdec.
   Qed.
 
-  Lemma strengthen_scoped : forall (t : S leaf) (X : Type) (γ1 γ2 : alist X) (k : K) (x : atom) (x' : X),
+  (** *** Strengthening *)
+  (******************************************************************************)
+  Lemma scoped_stren : forall (k : K) (t : S leaf) (X : Type) (γ1 γ2 : alist X) (x : atom) (x' : X),
       scoped S k t (domset (γ1 ++ x ~ x' ++ γ2)) ->
       ~ x ∈@ (freeset S k t) ->
       scoped S k t (domset (γ1 ++ γ2)).
@@ -98,442 +106,270 @@ Section scope_lemmas.
     autorewrite with tea_rw_dom in *. fsetdec.
   Qed.
 
-  Lemma sub_scoped :
-    forall (t1 : S leaf) (k : K) (t2 : T k leaf)
+  (** *** Substitution *)
+  (******************************************************************************)
+  Lemma scoped_sub_eq :
+    forall (k : K) (t1 : S leaf) (t2 : T k leaf)
       (X : Type) (γ1 γ2 : alist X) (x : atom) (x' : X),
       scoped S k t1 (domset (γ1 ++ x ~ x' ++ γ2)) ->
       scoped (T k) k t2 (domset (γ1 ++ γ2)) ->
       scoped S k (subst S k x t2 t1) (domset (γ1 ++ γ2)).
   Proof.
     introv hyp1 hyp2. unfold scoped in *. autorewrite with tea_rw_dom in *.
-    etransitivity.
-    (*
-      apply freeset_subst_upper_eq. fsetdec.
-     *)
-  Abort.
+    etransitivity. apply (freeset_subst_upper_eq S). fsetdec.
+  Qed.
 
-  Lemma sub_scoped_1 :
-    forall (t1 : S leaf) (k : K) (t2 : T k leaf)
-      (X : Type) (γ1 γ2 : alist X) (x : atom) (x' : X),
+  Lemma scoped_sub_neq :
+    forall (k1 k2 : K) (neq : k1 <> k2) (t1 : S leaf) (t2 : T k2 leaf)
+      (X : Type) (γ : alist X) (x : atom),
+      scoped S k1 t1 (domset γ) ->
+      scoped (T k2) k1 t2 (domset γ) ->
+      scoped S k1 (subst S k2 x t2 t1) (domset γ).
+  Proof.
+    introv hyp1 hyp2. unfold scoped in *. autorewrite with tea_rw_dom in *.
+    etransitivity. apply (freeset_subst_upper_neq S); auto. fsetdec.
+  Qed.
+
+  Lemma scoped_sub_eq1 :
+    forall (k : K) (t1 : S leaf) (t2 : T k leaf)
+      (X : Type) (γ1 : alist X) (x : atom) (x' : X),
       scoped S k t1 (domset (γ1 ++ x ~ x')) ->
       scoped (T k) k t2 (domset γ1) ->
       scoped S k (subst S k x t2 t1) (domset γ1).
   Proof.
-    (*
-    introv hyp1 hyp2. change_alist (γ ++ x ~ tt ++ []) in hyp1.
-    change_alist (γ ++ []) in hyp2.
-    change_alist (γ ++ []).
-    eauto using sub_scoped.
-     *)
-  Abort.
+    introv hyp1 hyp2. change_alist (γ1 ++ x ~ x' ++ []) in hyp1.
+    change_alist (γ1 ++ []) in hyp2.
+    change_alist (γ1 ++ []).
+    eauto using scoped_sub_eq.
+  Qed.
+
+  (** *** Other *)
+  (******************************************************************************)
+  Lemma scoped_envmap :
+    forall (k : K) (t1 : S leaf) (X Y : Type) (γ1 : alist X) (f : X -> Y),
+      scoped S k t1 (domset γ1) ->
+      scoped S k t1 (domset (envmap f γ1)).
+  Proof.
+    introv Hscope. unfold scoped in *.
+    now rewrite domset_fmap.
+  Qed.
 
 End scope_lemmas.
 
-(** ** Contexts of type variables (<<ok_tyv>>) *)
+(** * Infrastructural lemmas for contexts and well-formedness predicates *)
 (******************************************************************************)
-Lemma perm_ok_tyv : forall Δ1 Δ2,
-    ok_tyv Δ1 ->
+
+(** ** General properties of <<ok_kind_ctx>> *)
+(******************************************************************************)
+Lemma ok_kind_ctx_nil : forall x,
+    ok_kind_ctx [].
+Proof.
+  intros. unfold ok_kind_ctx in *.
+  now bursts.
+Qed.
+
+Lemma ok_kind_ctx_one : forall x,
+    ok_kind_ctx (x ~ tt).
+Proof.
+  intros. unfold ok_kind_ctx in *.
+  now bursts.
+Qed.
+
+Lemma ok_kind_ctx_app : forall Δ1 Δ2,
+    ok_kind_ctx (Δ1 ++ Δ2) <->
+    ok_kind_ctx Δ1 /\ ok_kind_ctx Δ2 /\ disjoint Δ1 Δ2.
+Proof.
+  intros. unfold ok_kind_ctx in *.
+  now bursts.
+Qed.
+
+Lemma ok_kind_ctx_comm : forall Δ1 Δ2,
+    ok_kind_ctx (Δ1 ++ Δ2) <->
+    ok_kind_ctx (Δ1 ++ Δ2).
+Proof.
+  intros. unfold ok_kind_ctx. bursts.
+  rewrite disjoint_sym. firstorder.
+Qed.
+
+Lemma ok_kind_ctx_perm1 : forall Δ1 Δ2,
+    ok_kind_ctx Δ1 ->
     Permutation Δ1 Δ2 ->
-    ok_tyv Δ2.
+    ok_kind_ctx Δ2.
 Proof.
-  unfold ok_tyv. intros. rewrite <- uniq_perm; eauto.
+  unfold ok_kind_ctx. intros. rewrite <- uniq_perm; eauto.
 Qed.
 
-#[export] Hint Immediate perm_ok_tyv : sysf_ctx.
-
-Corollary perm_ok_tyv_iff : forall Δ1 Δ2,
+Corollary ok_kind_ctx_perm : forall Δ1 Δ2,
     Permutation Δ1 Δ2 ->
-    ok_tyv Δ1 <-> ok_tyv Δ2.
+    ok_kind_ctx Δ1 <-> ok_kind_ctx Δ2.
 Proof.
-  unfold ok_tyv. intros. now rewrite uniq_perm.
+  unfold ok_kind_ctx. intros. now rewrite uniq_perm.
 Qed.
 
-Lemma ok_tyv_nil : forall x,
-    ok_tyv [].
+#[export] Hint Resolve ok_kind_ctx_nil : sysf_ctx.
+#[export] Hint Resolve ok_kind_ctx_one : sysf_ctx.
+#[export] Hint Immediate ok_kind_ctx_perm1 : sysf_ctx.
+
+(** ** Tactical support for <<ok_kind_ctx>> *)
+(******************************************************************************)
+Lemma ok_kind_ctx_app1 : forall Δ1 Δ2,
+    ok_kind_ctx Δ1 /\ ok_kind_ctx Δ2 /\ disjoint Δ1 Δ2 ->
+    ok_kind_ctx (Δ1 ++ Δ2).
 Proof.
-  intros. unfold ok_tyv in *.
+  intros. unfold ok_kind_ctx in *.
   now bursts.
 Qed.
 
-#[export] Hint Resolve ok_tyv_nil : sysf_ctx.
-
-Lemma ok_tyv_one : forall x,
-    ok_tyv (x ~ tt).
+Lemma ok_kind_ctx_mid1: forall Δ1 Δ2 Δ3,
+    ok_kind_ctx (Δ1 ++ Δ2 ++ Δ3) ->
+    ok_kind_ctx Δ2.
 Proof.
-  intros. unfold ok_tyv in *.
+  intros. unfold ok_kind_ctx in *.
   now bursts.
 Qed.
 
-#[export] Hint Resolve ok_tyv_one : sysf_ctx.
-
-Lemma ok_tyv_app_iff : forall Δ1 Δ2,
-    ok_tyv (Δ1 ++ Δ2) <->
-    ok_tyv Δ1 /\ ok_tyv Δ2 /\ disjoint Δ1 Δ2.
+Lemma ok_kind_ctx_mid2 : forall Δ1 Δ2 Δ3,
+    ok_kind_ctx (Δ1 ++ Δ2 ++ Δ3) ->
+    ok_kind_ctx (Δ1 ++ Δ3).
 Proof.
-  intros. unfold ok_tyv in *.
-  now bursts.
-Qed.
-
-Lemma ok_tyv_app_1 : forall Δ1 Δ2,
-    ok_tyv Δ1 /\ ok_tyv Δ2 /\ disjoint Δ1 Δ2 ->
-    ok_tyv (Δ1 ++ Δ2).
-Proof.
-  intros. unfold ok_tyv in *.
-  now bursts.
-Qed.
-
-#[export] Hint Resolve ok_tyv_app_1 : sysf_ctx.
-
-Lemma ok_tyv_mid_1: forall Δ1 Δ2 Δ3,
-    ok_tyv (Δ1 ++ Δ2 ++ Δ3) ->
-    ok_tyv Δ2.
-Proof.
-  intros. unfold ok_tyv in *.
-  now bursts.
-Qed.
-
-Lemma ok_tyv_mid_2 : forall Δ1 Δ2 Δ3,
-    ok_tyv (Δ1 ++ Δ2 ++ Δ3) ->
-    ok_tyv (Δ1 ++ Δ3).
-Proof.
-  intros. unfold ok_tyv in *.
+  intros. unfold ok_kind_ctx in *.
   bursts. now rewrite disjoint_sym.
 Qed.
 
-Lemma ok_tyv_app_l : forall Δ1 Δ2,
-    ok_tyv (Δ1 ++ Δ2) ->
-    ok_tyv Δ1.
+Lemma ok_kind_ctx_app_l : forall Δ1 Δ2,
+    ok_kind_ctx (Δ1 ++ Δ2) ->
+    ok_kind_ctx Δ1.
 Proof.
-  intros. unfold ok_tyv in *.
+  intros. unfold ok_kind_ctx in *.
   now bursts.
 Qed.
 
-Lemma ok_tyv_app_r : forall Δ1 Δ2,
-    ok_tyv (Δ1 ++ Δ2) ->
-    ok_tyv Δ2.
+Lemma ok_kind_ctx_app_r : forall Δ1 Δ2,
+    ok_kind_ctx (Δ1 ++ Δ2) ->
+    ok_kind_ctx Δ2.
 Proof.
-  intros. unfold ok_tyv in *.
+  intros. unfold ok_kind_ctx in *.
   now bursts.
 Qed.
 
-#[export] Hint Immediate ok_tyv_mid_1 ok_tyv_mid_2 : sysf_ctx.
-#[export] Hint Immediate ok_tyv_app_l ok_tyv_app_r : sysf_ctx.
+#[export] Hint Resolve ok_kind_ctx_app1 : sysf_ctx.
+#[export] Hint Immediate ok_kind_ctx_mid1 ok_kind_ctx_mid2 : sysf_ctx.
+#[export] Hint Immediate ok_kind_ctx_app_l ok_kind_ctx_app_r : sysf_ctx.
 
-(** ** Well-scoped types in context Δ *)
-(** A type is well-scoped in a type-variable environment when all of
-    its free variables (which are always type variables) are declared
-    in the context. Such a type may or may not be locally
-    closed. Well-scopedness is preserved under permutation, weakening,
-    and strengthening. It also satisfies a substitution lemma. *)
+(** ** General properties of <<ok_type>> *)
 (******************************************************************************)
-(*
-(** The <<scoped_type>> predicate supports permutation in Δ. *)
-Lemma perm_scoped_type : forall Δ1 Δ2 τ,
-    Permutation Δ1 Δ2 ->
-    scoped_type Δ1 τ <->
-    scoped_type Δ2 τ.
-Proof.
-  intros. unfold scoped_type. apply perm_scoped_iff; auto.
-Qed.
 
-(** The <<scoped_type>> predicate supports weakening in Δ. *)
-Lemma weak_scoped_type_r : forall Δ1 Δ2 τ,
-    scoped_type Δ1 τ ->
-    scoped_type (Δ1 ++ Δ2) τ.
-Proof.
-  intros. unfold scoped_type in *.
-  now apply weak_scoped_app_l.
-Qed.
-
-Lemma weak_scoped_type_l : forall Δ1 Δ2 τ,
-    scoped_type Δ2 τ ->
-    scoped_type (Δ1 ++ Δ2) τ.
-Proof.
-  intros. unfold scoped_type in *.
-  now apply weak_scoped_app_r.
-Qed.
-
-(** The <<scoped_type>> predicate supports strengthening in Δ for fresh variables. *)
-Lemma stren_scoped_type : forall Δ1 Δ2 x τ,
-    scoped_type (Δ1 ++ x ~ tt ++ Δ2) τ ->
-    ~ x ∈@ (freeset typ KType τ) ->
-    scoped_type (Δ1 ++ Δ2) τ.
-Proof.
-  introv hyp hnotin. unfold scoped_type in *.
-  eapply stren_scoped; eauto.
-Qed.
-
-Corollary stren_scoped_type_1 : forall Δ x τ,
-    scoped_type (Δ ++ x ~ tt) τ ->
-    ~ x ∈@ (freeset typ KType τ) ->
-    scoped_type Δ τ.
-Proof.
-  introv H1 H2. change_alist (Δ ++ x ~ tt ++ []) in H1.
-  change_alist (Δ ++ []). eauto using stren_scoped_type.
-Qed.
-
-(** The <<scoped_type>> predicate supports substitution w.r.t. in Δ. *)
-Lemma sub_scoped_type : forall Δ1 Δ2 x τ1 τ2,
-    scoped_type (Δ1 ++ x ~ tt ++ Δ2) τ1 ->
-    scoped_type (Δ1 ++ Δ2) τ2 ->
-    scoped_type (Δ1 ++ Δ2) (subst typ KType x τ2 τ1).
-Proof.
-  intros. apply sub_scoped; auto.
-Qed.
-
-Corollary sub_scoped_type_1 : forall Δ x τ1 τ2,
-    scoped_type (Δ ++ x ~ tt) τ1 ->
-    scoped_type Δ τ2 ->
-    scoped_type Δ (subst typ KType x τ2 τ1).
-Proof.
-  introv H1 H2. change_alist (Δ ++ x ~ tt ++ []) in H1.
-  change_alist (Δ ++ []) in H2. change_alist (Δ ++ []).
-  auto using sub_scoped_type.
-Qed.
-
-#[export] Hint Resolve weak_scoped_type_l weak_scoped_type_r perm_scoped_type
- stren_scoped_type stren_scoped_type_1 sub_scoped_type sub_scoped_type_1 : tea_sysf.
- *)
-
-(** ** Well-formed type expressions (<<ok_type>>) *)
-(******************************************************************************)
-Corollary ok_type_lc : forall Δ τ,
+(** A well-formed type is locally closed. *)
+Lemma ok_type_lc : forall Δ τ,
     ok_type Δ τ ->
     locally_closed typ KType τ.
 Proof.
   unfold ok_type. tauto.
 Qed.
 
+#[export] Hint Immediate ok_type_lc : sysf_ctx.
 #[export] Hint Resolve ok_type_lc : sysf_ctx.
 
-Lemma perm_ok_type : forall Δ1 Δ2 τ,
+(** ** Structural properties of <<ok_type Δ τ>> in <<Δ>> *)
+(******************************************************************************)
+
+(** *** Permutation *)
+Lemma ok_type_perm : forall Δ1 Δ2 τ,
     Permutation Δ1 Δ2 ->
     ok_type Δ1 τ <->
     ok_type Δ2 τ.
 Proof.
-  intros. unfold ok_type. rewrite (perm_scoped_iff _ _); eauto.
-  reflexivity.
+  intros. unfold ok_type. now rewrite (scoped_perm); eauto.
 Qed.
 
-Lemma perm_ok_type_1 : forall Δ1 Δ2 τ,
+Lemma ok_type_perm1 : forall Δ1 Δ2 τ,
     ok_type Δ1 τ ->
     Permutation Δ1 Δ2 ->
     ok_type Δ2 τ.
 Proof.
-  intros. rewrite <- perm_ok_type; eauto.
+  intros. rewrite <- ok_type_perm; eauto.
 Qed.
 
-#[export] Hint Immediate perm_ok_type_1 : sysf_ctx.
-
-(** The <<ok_type>> predicate supports weakening in Δ. *)
-(* TODO: Understand how to prevent
-    auto using weak_scoped_app_l diverges. *)
-Lemma weak_ok_type_r : forall Δ1 Δ2 τ,
+(** *** Weakening *)
+Lemma ok_type_weak_r : forall Δ1 Δ2 τ,
     ok_type Δ1 τ ->
     ok_type (Δ1 ++ Δ2) τ.
 Proof.
   unfold ok_type.
   intros. split.
-  - Check weak_scoped_app_l typ.
-    apply (weak_scoped_app_l typ).
+  - apply (scoped_weak_l typ). tauto.
   - tauto.
-  intuition (eauto using (weak_scoped_app_l typ)).
 Qed.
 
-Lemma weak_ok_type_l : forall Δ1 Δ2 τ,
+Lemma ok_type_weak_l : forall Δ1 Δ2 τ,
     ok_type Δ2 τ ->
     ok_type (Δ1 ++ Δ2) τ.
 Proof.
-  unfold ok_type. intuition (auto using (weak_scoped_app_r (F:=typ))).
+  unfold ok_type. intuition (auto using (scoped_weak_r typ)).
 Qed.
 
-#[export] Hint Resolve weak_ok_type_l weak_ok_type_r : sysf_ctx.
-
-(** The <<ok_type>> predicate supports strengthening in Δ for fresh variables. *)
-Lemma stren_ok_type : forall Δ1 Δ2 x τ,
+(** *** Strengthening  *)
+Lemma ok_type_stren : forall Δ1 Δ2 x τ,
     ok_type (Δ1 ++ x ~ tt ++ Δ2) τ ->
     ~ x ∈@ (freeset typ KType τ) ->
     ok_type (Δ1 ++ Δ2) τ.
 Proof.
   introv [? ?] ?. unfold ok_type.
-  eauto using (stren_scoped (F:=typ)).
+  eauto using (scoped_stren typ).
 Qed.
 
-Corollary stren_ok_type_1 : forall Δ x τ,
+Corollary ok_type_stren1 : forall Δ x τ,
     ok_type (Δ ++ x ~ tt) τ ->
     ~ x ∈@ (freeset typ KType τ) ->
     ok_type Δ τ.
 Proof.
   introv H1 H2. change_alist (Δ ++ x ~ tt ++ []) in H1.
-  change_alist (Δ ++ []). eauto using stren_ok_type.
+  change_alist (Δ ++ []). eauto using ok_type_stren.
 Qed.
 
-#[export] Hint Immediate stren_ok_type stren_ok_type_1 : sysf_ctx.
-
-(** The <<ok_type>> predicate supports substitution w.r.t. in Δ. *)
-Lemma sub_ok_type : forall Δ1 Δ2 x τ1 τ2,
+(** *** Substitution *)
+Lemma ok_type_sub : forall Δ1 Δ2 x τ1 τ2,
     ok_type (Δ1 ++ x ~ tt ++ Δ2) τ1 ->
     ok_type (Δ1 ++ Δ2) τ2 ->
     ok_type (Δ1 ++ Δ2) (subst typ KType x τ2 τ1).
 Proof.
   unfold ok_type. introv [? ?] [? ?]. split.
-  - auto using (sub_scoped (F:=typ)).
-  - auto using (subst_lc_eq (F:=typ)).
+  - pose (lemma := scoped_sub_eq typ KType).
+    eapply lemma; eassumption.
+  - auto using (subst_lc_eq typ).
 Qed.
 
-#[export] Hint Resolve sub_ok_type : sysf_ctx.
-
-Corollary sub_ok_type_1 : forall Δ x τ1 τ2,
+Corollary ok_type_sub1 : forall Δ x τ1 τ2,
     ok_type (Δ ++ x ~ tt) τ1 ->
     ok_type Δ τ2 ->
     ok_type Δ (subst typ KType x τ2 τ1).
 Proof.
   introv H1 H2. change_alist (Δ ++ x ~ tt ++ []) in H1.
   change_alist (Δ ++ []) in H2. change_alist (Δ ++ []).
-  auto using sub_ok_type.
+  auto using ok_type_sub.
 Qed.
 
-#[export] Hint Resolve sub_ok_type_1 : sysf_ctx.
+#[export] Hint Immediate ok_type_perm1 : sysf_ctx.
+#[export] Hint Resolve ok_type_weak_l ok_type_weak_r : sysf_ctx.
+#[export] Hint Immediate ok_type_stren ok_type_stren1 : sysf_ctx.
+#[export] Hint Resolve ok_type_sub : sysf_ctx.
+#[export] Hint Resolve ok_type_sub1 : sysf_ctx.
 
-(** * Term variable contexts *)
-(** Contexts of <<free term variable, type>> assigments), used to declare free term
-    variables and their associated typee. *)
+(** ** General properties of <<ok_type_ctx>> *)
 (******************************************************************************)
-
-(** A term-variable context <<Γ>> is well formed in type-variable
-    context <<Δ>> when it is duplicate-free and each type is well
-    formed in <<Δ>>. The [ok_tmv] judgment is preserved under
-    permutation of <<Γ>>, and preserved under permutation, weakening,
-    strengthening, and substitution in <<Δ>>.*)
-
-(** ** Structural properties of <<Δ>> in <<ok_tmv Δ Γ>>. *)
-Corollary binds_ok_tmv : forall Δ Γ x τ,
-    ok_tmv Δ Γ ->
-    (x, τ) ∈ Γ ->
-    ok_type Δ τ.
+Lemma ok_type_ctx_nil : forall Δ,
+    ok_type_ctx Δ [].
 Proof.
-  introv ? Hin. unfold ok_tmv, ok_type in *.
-  apply binds_in_range in Hin. firstorder.
+  intros. unfold ok_type_ctx in *. now bursts.
 Qed.
 
-#[export] Hint Immediate binds_ok_tmv : sysf_ctx.
-
-(** The <<ok_tmv>> predicate supports permutation in Δ. *)
-Theorem perm_ok_tmv : forall Δ1 Δ2 Γ,
-    ok_tmv Δ1 Γ ->
-    Permutation Δ1 Δ2 ->
-    ok_tmv Δ2 Γ.
-Proof.
-  introv [? ?] ?. unfold ok_tmv.
-  split; eauto using perm_ok_type_1 with tea_alist.
-Qed.
-
-#[export] Hint Immediate perm_ok_tmv : sysf_ctx.
-
-Corollary perm_ok_tmv_iff : forall Δ1 Δ2 Γ,
-    Permutation Δ1 Δ2 ->
-    ok_tmv Δ1 Γ <-> ok_tmv Δ2 Γ.
-Proof.
-  introv Hperm. unfold ok_tmv, ok_type.
-  assert (lemma : forall τ, scoped_env typ KType τ Δ1 <->
-                            scoped_env typ KType τ Δ2).
-  { intros. now rewrite perm_scoped_iff. }
-  (* todo : figure out why <<perm_scoped_iff>> won't rewrite by itself. *)
-  setoid_rewrite lemma. firstorder.
-Qed.
-
-(** The <<ok_tmv>> predicate supports weakening in <<Δ>>. *)
-
-#[local] Set Firstorder Depth 4.
-
-Lemma weak_ok_tmv : forall Δ1 Δ2 Γ,
-    ok_tmv Δ1 Γ ->
-    ok_tmv (Δ1 ++ Δ2) Γ.
-Proof.
-  introv [huniq hok1]. unfold ok_tmv in *.
-  firstorder using weak_ok_type_r.
-Qed.
-
-#[export] Hint Resolve weak_ok_tmv : sysf_ctx.
-
-(** The <<ok_tmv>> predicate supports strengthening in <<Δ>> for fresh variables. *)
-Lemma stren_ok_tmv : forall Δ1 Δ2 x Γ,
-    ok_tmv (Δ1 ++ x ~ tt ++ Δ2) Γ ->
-    ~ x ∈@ freeset (fun A => alist typ A) KType Γ ->
-    ok_tmv (Δ1 ++ Δ2) Γ.
-Proof.
-  introv [hunit hok] hfresh. rewrite nin_freeset_iff in hfresh.
-  unfold ok_tmv. split; [trivial |].
-  intros τ hin; specialize (hok τ hin).
-  intuition (eauto using stren_ok_type).
-Qed.
-
-Corollary stren_ok_tmv_1 : forall Δ x Γ,
-    ok_tmv (Δ ++ x ~ tt) Γ ->
-    ~ x ∈@ freeset (fun A => alist typ A) KType Γ ->
-    ok_tmv Δ Γ.
-Proof.
-  introv hyp1 hyp2. change_alist (Δ ++ x ~ tt ++ []) in hyp1.
-  change_alist (Δ ++ []). eauto using stren_ok_tmv.
-Qed.
-
-(** The <<ok_tmv>> predicate supports substitution w.r.t. <<Δ>> *)
-Lemma sub_ok_tmv : forall Δ1 Δ2 x Γ τ,
-    ok_tmv (Δ1 ++ x ~ tt ++ Δ2) Γ ->
-    ok_type (Δ1 ++ Δ2) τ ->
-    locally_closed typ KType τ ->
-    ok_tmv (Δ1 ++ Δ2) (subst (fun A => alist typ A) KType x τ Γ).
-Proof.
-  introv [hunit hok] Hscope lc. unfold ok_tmv. split.
-  - now rewrite <- uniq_subst.
-  - intros τ2 τ2in. rewrite in_range_subst in τ2in.
-    destruct τ2in as [τ2_inv [hin ?]]; subst.
-    specialize (hok τ2_inv hin).
-    auto using sub_ok_type.
-Qed.
-
-#[export] Hint Resolve sub_ok_tmv : sysf_ctx.
-
-(** ** Structural properties of <<Γ>> in <<ok_tmv Δ Γ>>. *)
-
-(** <<ok_tmv Δ Γ>> supports permutation in Γ. *)
-Lemma perm_tm_ok_tmv : forall Δ Γ1 Γ2,
-    ok_tmv Δ Γ1 ->
-    Permutation Γ1 Γ2 ->
-    ok_tmv Δ Γ2.
-Proof.
-  introv [huniq hok]. unfold ok_tmv in *. split.
-  - rewrite uniq_perm; eauto. now symmetry.
-  - intros τ hin; specialize (hok τ).
-    apply hok. rewrite perm_range; eauto.
-Qed.
-
-#[export] Hint Immediate perm_tm_ok_tmv : sysf_ctx.
-
-Corollary perm_tm_ok_tmv_iff : forall Δ Γ1 Γ2,
-    Permutation Γ1 Γ2 ->
-    ok_tmv Δ Γ1 <-> ok_tmv Δ Γ2.
-Proof.
-  introv Hperm; split; intro.
-  - eauto using perm_tm_ok_tmv.
-  - symmetry in Hperm. eauto using perm_tm_ok_tmv.
-Qed.
-
-Lemma ok_tmv_tm_nil : forall Δ,
-    ok_tmv Δ [].
-Proof.
-  intros. unfold ok_tmv in *. now bursts.
-Qed.
-
-#[export] Hint Resolve ok_tmv_tm_nil : sysf_ctx.
-
-Lemma ok_tmv_tm_cons : forall Δ Γ x τ,
-    ok_tmv Δ Γ ->
+Lemma ok_type_ctx_cons : forall Δ Γ x τ,
+    ok_type_ctx Δ Γ ->
     ~ (x ∈@ domset Γ) ->
     ok_type Δ τ ->
-    ok_tmv Δ (x ~ τ ++ Γ).
+    ok_type_ctx Δ (x ~ τ ++ Γ).
 Proof.
-  intros. unfold ok_tmv in *. bursts.
+  intros. unfold ok_type_ctx in *. bursts.
   splits.
   - intuition.
   - intros ? [?|?].
@@ -541,75 +377,295 @@ Proof.
     + firstorder.
 Qed.
 
-#[export] Hint Resolve ok_tmv_tm_cons : sysf_ctx.
-
-Lemma ok_tmv_tm_one : forall Δ x τ,
+Lemma ok_type_ctx_one : forall Δ x τ,
     ok_type Δ τ ->
-    ok_tmv Δ (x ~ τ).
+    ok_type_ctx Δ (x ~ τ).
 Proof.
   intros. change (x ~ τ) with [(x, τ)].
-  apply ok_tmv_tm_cons; auto using ok_tmv_tm_nil.
+  apply ok_type_ctx_cons; auto using ok_type_ctx_nil.
   fsetdec.
 Qed.
 
-#[export] Hint Resolve ok_tmv_tm_one : sysf_ctx.
-
-Lemma ok_tmv_tm_app : forall Δ Γ1 Γ2,
-    ok_tmv Δ (Γ1 ++ Γ2) <->
-    ok_tmv Δ Γ1 /\ ok_tmv Δ Γ2 /\ disjoint Γ1 Γ2.
+Lemma ok_type_ctx_app : forall Δ Γ1 Γ2,
+    ok_type_ctx Δ (Γ1 ++ Γ2) <->
+    ok_type_ctx Δ Γ1 /\ ok_type_ctx Δ Γ2 /\ disjoint Γ1 Γ2.
 Proof.
-  intros. unfold ok_tmv.
+  intros. unfold ok_type_ctx.
   setoid_rewrite in_range_iff.
   setoid_rewrite List.in_list_app.
   rewrite uniq_app_iff. firstorder.
 Qed.
 
-Lemma ok_tmv_inv_app_l : forall Δ Γ1 Γ2,
-    ok_tmv Δ (Γ1 ++ Γ2) ->
-    ok_tmv Δ Γ1.
+Lemma ok_type_ctx_app_comm : forall {Δ Γ1 Γ2},
+    ok_type_ctx Δ (Γ1 ++ Γ2) <->
+    ok_type_ctx Δ (Γ2 ++ Γ1).
 Proof.
-  introv [huniq hscope]. unfold ok_tmv in *.
-  bursts. firstorder.
-Qed.
-
-#[export] Hint Immediate ok_tmv_inv_app_l : sysf_ctx.
-
-Lemma ok_tmv_app_comm : forall {Δ Γ1 Γ2},
-    ok_tmv Δ (Γ1 ++ Γ2) <->
-    ok_tmv Δ (Γ2 ++ Γ1).
-Proof.
-  intros. unfold ok_tmv. bursts.
+  intros. unfold ok_type_ctx. bursts.
   rewrite disjoint_sym. firstorder.
 Qed.
 
-#[export] Hint Immediate ok_tmv_app_comm : sysf_ctx.
-
-Corollary ok_tmv_inv_app_r : forall Δ Γ1 Γ2,
-    ok_tmv Δ (Γ1 ++ Γ2) ->
-    ok_tmv Δ Γ2.
+Lemma ok_type_ctx_binds : forall Δ Γ x τ,
+    ok_type_ctx Δ Γ ->
+    (x, τ) ∈ Γ ->
+    ok_type Δ τ.
 Proof.
-  introv hyp. rewrite ok_tmv_app_comm in hyp.
-  eauto using ok_tmv_inv_app_l.
+  introv Hok Hin. unfold ok_type_ctx, ok_type in *.
+  apply Hok. erewrite (in_range_iff Γ); eauto.
 Qed.
 
-#[export] Hint Immediate ok_tmv_inv_app_r : sysf_ctx.
+(** <<ok_type_ctx Δ Γ>> supports permutation in Γ. *)
+Lemma ok_type_ctx_perm_gamma1 : forall Δ Γ1 Γ2,
+    ok_type_ctx Δ Γ1 ->
+    Permutation Γ1 Γ2 ->
+    ok_type_ctx Δ Γ2.
+Proof.
+  introv [huniq hok]. unfold ok_type_ctx in *. split.
+  - rewrite uniq_perm; eauto. now symmetry.
+  - intros τ hin; specialize (hok τ).
+    apply hok. rewrite perm_range; eauto.
+Qed.
 
-Corollary ok_tmv_inv_mid : forall Δ Γ1 Γ2 Γ3,
-    ok_tmv Δ (Γ1 ++ Γ2 ++ Γ3) ->
-    ok_tmv Δ (Γ1 ++ Γ3).
+Corollary ok_type_ctx_perm_gamma : forall Δ Γ1 Γ2,
+    Permutation Γ1 Γ2 ->
+    ok_type_ctx Δ Γ1 <-> ok_type_ctx Δ Γ2.
+Proof.
+  introv Hperm; split; intro.
+  - eauto using ok_type_ctx_perm_gamma1.
+  - symmetry in Hperm. eauto using ok_type_ctx_perm_gamma1.
+Qed.
+
+#[export] Hint Resolve ok_type_ctx_nil : sysf_ctx.
+#[export] Hint Resolve ok_type_ctx_cons : sysf_ctx.
+#[export] Hint Resolve ok_type_ctx_one : sysf_ctx.
+#[export] Hint Immediate ok_type_ctx_app_comm : sysf_ctx.
+#[export] Hint Immediate ok_type_ctx_binds : sysf_ctx.
+#[export] Hint Immediate ok_type_ctx_perm_gamma : sysf_ctx.
+
+(** ** Tactical support for <<ok_type_ctx>> *)
+(******************************************************************************)
+Lemma ok_type_ctx_inv_app_l : forall Δ Γ1 Γ2,
+    ok_type_ctx Δ (Γ1 ++ Γ2) ->
+    ok_type_ctx Δ Γ1.
+Proof.
+  introv [huniq hscope]. unfold ok_type_ctx in *.
+  bursts. firstorder.
+Qed.
+
+Corollary ok_type_ctx_inv_app_r : forall Δ Γ1 Γ2,
+    ok_type_ctx Δ (Γ1 ++ Γ2) ->
+    ok_type_ctx Δ Γ2.
+Proof.
+  introv hyp. rewrite ok_type_ctx_app_comm in hyp.
+  eauto using ok_type_ctx_inv_app_l.
+Qed.
+
+Corollary ok_type_ctx_inv_mid : forall Δ Γ1 Γ2 Γ3,
+    ok_type_ctx Δ (Γ1 ++ Γ2 ++ Γ3) ->
+    ok_type_ctx Δ (Γ1 ++ Γ3).
 Proof.
   introv hyp.
   change_alist ((Γ1 ++ Γ2) ++ Γ3) in hyp.
-  rewrite ok_tmv_app_comm in hyp.
+  rewrite ok_type_ctx_app_comm in hyp.
   change_alist ((Γ3 ++ Γ1) ++ Γ2) in hyp.
-  apply ok_tmv_inv_app_l in hyp.
-  now rewrite ok_tmv_app_comm in hyp.
+  apply ok_type_ctx_inv_app_l in hyp.
+  now rewrite ok_type_ctx_app_comm in hyp.
 Qed.
 
-#[export] Hint Immediate ok_tmv_inv_mid : sysf_ctx.
+#[export] Hint Immediate ok_type_ctx_inv_app_l : sysf_ctx.
+#[export] Hint Immediate ok_type_ctx_inv_app_r : sysf_ctx.
+#[export] Hint Immediate ok_type_ctx_inv_mid : sysf_ctx.
 
-(** * Well-formed terms, <<Δ ; Γ ⊢ t OK>> *)
+(** ** Structural properties in <<Δ>> in <<ok_type_ctx Δ Γ>>. *)
+(******************************************************************************)
 
-(** ** Structural properties of <<Δ>> in <<Δ ; Γ ⊢ t OK>>. *)
+(** *** Permutation *)
+Theorem ok_type_ctx_perm1 : forall Δ1 Δ2 Γ,
+    ok_type_ctx Δ1 Γ ->
+    Permutation Δ1 Δ2 ->
+    ok_type_ctx Δ2 Γ.
+Proof.
+  introv [? ?] ?. unfold ok_type_ctx.
+  split; eauto using ok_type_perm1 with tea_alist.
+Qed.
 
-(** ** Structural properties of <<Γ>> in <<Δ ; Γ ⊢ t : τ>>. *)
+Corollary ok_type_ctx_perm : forall Δ1 Δ2 Γ,
+    Permutation Δ1 Δ2 ->
+    ok_type_ctx Δ1 Γ <-> ok_type_ctx Δ2 Γ.
+Proof.
+  introv Hperm. unfold ok_type_ctx, ok_type.
+  split; intros.
+  - eapply ok_type_ctx_perm1; eauto.
+  - eapply ok_type_ctx_perm1; eauto.
+    now apply Permutation_sym.
+Qed.
+
+#[local] Set Firstorder Depth 4.
+
+(** *** Weakening *)
+Lemma ok_type_ctx_weak_r : forall Δ1 Δ2 Γ,
+    ok_type_ctx Δ1 Γ ->
+    ok_type_ctx (Δ1 ++ Δ2) Γ.
+Proof.
+  introv [huniq hok1]. unfold ok_type_ctx in *.
+  firstorder using ok_type_weak_r.
+Qed.
+
+(** *** Strengthening *)
+Lemma ok_type_ctx_stren : forall Δ1 Δ2 x Γ,
+    ok_type_ctx (Δ1 ++ x ~ tt ++ Δ2) Γ ->
+    (forall t : typ leaf, t ∈ range Γ -> ~ x ∈@ freeset typ KType t) ->
+    ok_type_ctx (Δ1 ++ Δ2) Γ.
+Proof.
+  introv [hunit hok] hfresh.
+  unfold ok_type_ctx. split; [trivial |].
+  intros τ hin; specialize (hok τ hin).
+  eauto using ok_type_stren.
+Qed.
+
+Corollary ok_type_ctx_stren1 : forall Δ x Γ,
+    ok_type_ctx (Δ ++ x ~ tt) Γ ->
+    (forall t : typ leaf, t ∈ range Γ -> ~ x ∈@ freeset typ KType t) ->
+    ok_type_ctx Δ Γ.
+Proof.
+  introv hyp1 hyp2. change_alist (Δ ++ x ~ tt ++ []) in hyp1.
+  change_alist (Δ ++ []). eauto using ok_type_ctx_stren.
+Qed.
+
+Lemma ok_type_ctx_sub : forall Δ1 Δ2 x Γ τ,
+    ok_type_ctx (Δ1 ++ x ~ tt ++ Δ2) Γ ->
+    ok_type (Δ1 ++ Δ2) τ ->
+    locally_closed typ KType τ ->
+    ok_type_ctx (Δ1 ++ Δ2) (envmap (subst typ KType x τ) Γ).
+Proof.
+  introv [hunit hok] Hscope lc. unfold ok_type_ctx. split.
+  - now apply uniq_fmap2.
+  - intros τ2 τ2in.
+    rewrite in_range_iff in τ2in.
+    setoid_rewrite in_envmap_iff in τ2in.
+    destruct τ2in as [y [τ2_inv [? ?]]]; subst.
+    specialize (hok τ2_inv).
+    apply ok_type_sub.
+    + apply hok. rewrite in_range_iff. eauto.
+    + auto.
+Qed.
+
+#[export] Hint Immediate ok_type_ctx_perm : sysf_ctx.
+#[export] Hint Resolve ok_type_ctx_perm1 : sysf_ctx.
+#[export] Hint Resolve ok_type_ctx_weak_r : sysf_ctx.
+#[export] Hint Resolve ok_type_ctx_sub : sysf_ctx.
+
+(** ** Structural properties of <<ok_term Δ Γ t>> in <<Δ>> *)
+(******************************************************************************)
+
+(** *** Permutation *)
+Lemma ok_term_perm_delta : forall Δ1 Δ2 Γ t,
+    Permutation Δ1 Δ2 ->
+    ok_term Δ1 Γ t <->
+    ok_term Δ2 Γ t.
+Proof.
+  intros. unfold ok_term.
+  now rewrite scoped_perm.
+Qed.
+
+(** *** Weakening *)
+Lemma ok_term_weak_delta_r : forall Δ1 Δ2 Γ t,
+    ok_term Δ1 Γ t ->
+    ok_term (Δ1 ++ Δ2) Γ t.
+Proof.
+  unfold ok_term. intros.
+  intuition (eauto using (scoped_weak_l term)).
+Qed.
+
+Lemma ok_term_weak_delta_l : forall Δ1 Δ2 Γ t,
+    ok_term Δ2 Γ t ->
+    ok_term (Δ1 ++ Δ2) Γ t.
+Proof.
+  unfold ok_term. intros.
+  intuition (eauto using (scoped_weak_r term)).
+Qed.
+
+(** *** Strengthening  *)
+Lemma ok_term_stren_delta : forall Δ1 Δ2 x Γ t,
+    ok_term (Δ1 ++ x ~ tt ++ Δ2) Γ t ->
+    ~ x ∈@ (freeset term KType t) ->
+    ok_term (Δ1 ++ Δ2) Γ t.
+Proof.
+  introv Hok Hfresh. unfold ok_term in *.
+  intuition. eapply (scoped_stren term); eauto.
+Qed.
+
+(** *** Substitution *)
+Lemma ok_term_sub_delta : forall Δ1 Δ2 x τ Γ t,
+    ok_term (Δ1 ++ x ~ tt ++ Δ2) Γ t ->
+    ok_type (Δ1 ++ Δ2) τ ->
+    ok_term (Δ1 ++ Δ2) (envmap (subst typ KType x τ) Γ) (subst term KType x τ t).
+Proof.
+  introv Hokt Hokτ. unfold ok_term, ok_type in *.
+  intuition.
+  - eapply (scoped_sub_eq term); eauto.
+  - apply scoped_envmap.
+    eapply (scoped_sub_neq term); eauto.
+    + discriminate.
+    + apply rw_scoped_KTerm_type.
+  - eapply (subst_lc_neq term); auto.
+    + discriminate.
+    + apply rw_lc_KTerm_type.
+  - eapply (subst_lc_eq term); auto.
+Qed.
+
+(** ** Structural properties of <<ok_term Δ Γ t>> in <<Γ>> *)
+(******************************************************************************)
+
+(** *** Permutation *)
+Lemma ok_term_perm_gamma : forall Δ Γ1 Γ2 t,
+    Permutation Γ1 Γ2 ->
+    ok_term Δ Γ1 t <->
+    ok_term Δ Γ2 t.
+Proof.
+  intros. unfold ok_term.
+  pose (lemma := scoped_perm term (KTerm : K)).
+  now rewrite lemma; eauto.
+Qed.
+
+(** *** Weakening *)
+Lemma ok_term_weak_gamma_r : forall Δ Γ1 Γ2 t,
+    ok_term Δ Γ1 t ->
+    ok_term Δ (Γ1 ++ Γ2) t.
+Proof.
+  unfold ok_term. intros.
+  intuition (eauto using (scoped_weak_l term)).
+Qed.
+
+Lemma ok_term_weak_gamma_l : forall Δ Γ1 Γ2 t,
+    ok_term Δ Γ2 t ->
+    ok_term Δ (Γ1 ++ Γ2) t.
+Proof.
+  unfold ok_term. intros.
+  intuition (eauto using (scoped_weak_r term)).
+Qed.
+
+(** *** Strengthening  *)
+Lemma ok_term_stren_gamma : forall Δ Γ1 Γ2 x τ t,
+    ok_term Δ (Γ1 ++ x ~ τ ++ Γ2) t ->
+    ~ x ∈@ (freeset term KTerm t) ->
+    ok_term Δ (Γ1 ++ Γ2) t.
+Proof.
+  introv Hok Hfresh. unfold ok_term in *.
+  intuition. eapply (scoped_stren term); eauto.
+Qed.
+
+(** *** Substitution *)
+Lemma ok_term_sub_gamma : forall Δ Γ1 Γ2 x τ u t,
+    ok_term Δ (Γ1 ++ x ~ τ ++ Γ2) t ->
+    ok_term Δ (Γ1 ++ Γ2) u ->
+    ok_term Δ (Γ1 ++ Γ2) (subst term KTerm x u t).
+Proof.
+  introv Hokt Hoku. unfold ok_term, ok_type in *.
+  intuition.
+  - eapply (scoped_sub_neq term); auto.
+    + discriminate.
+  - eapply (scoped_sub_eq term); eauto.
+  - eapply (subst_lc_eq term); auto.
+  - eapply (subst_lc_neq term); auto.
+    + discriminate.
+Qed.
