SystemF/Rewriting.v
@@ -1,0 +1,838 @@
+From Tealeaves Require Import
+     Functors.List
+     LN.Leaf LN.Atom LN.AtomSet LN.AssocList
+     LN.Multisorted.Operations.
+
+From Multisorted Require Import
+     Classes.DTM
+     Theory.DTMContainer
+     Theory.DTMSchedule.
+
+From Tealeaves.Examples Require Import
+     SystemF.Language.
+
+Import DTMContainer.Notations.
+Import AtomSet.Notations.
+Import Tealeaves.Classes.Monoid.Notations.
+Import Tealeaves.Theory.Product.Notations.
+Import Tealeaves.Classes.Applicative.Notations.
+Import Multisorted.Classes.DTM.Notations.
+Import List.ListNotations.
+Import SetlikeFunctor.Notations.
+
+Open Scope set_scope.
+Open Scope list_scope.
+Open Scope tealeaves_scope.
+Open Scope tealeaves_multi_scope.
+
+(** * Rewriting rules for operations *)
+(******************************************************************************)
+
+Create HintDb sysf_rw.
+Tactic Notation "simpl_F" := autorewrite with sysf_rw.
+
+(** * Rewriting operations on <<typ>> *)
+(******************************************************************************)
+
+(** ** Fundamental operations *)
+(******************************************************************************)
+
+(** *** <<mbinddt>> *)
+(******************************************************************************)
+Section rw_mbinddt_type.
+
+  Context
+    (A B : Type)
+    `{Applicative F}
+    (f : forall k, list K * A -> F (SystemF k B)).
+
+  Lemma rw_mbinddt_type1 : forall c, mbinddt typ F f (ty_c c) = pure F (ty_c c).
+  Proof. reflexivity. Qed.
+
+  Lemma rw_mbinddt_type2 : forall (a : A), mbinddt typ F f (ty_v a) = f KType (nil, a).
+  Proof. reflexivity. Qed.
+
+  Lemma rw_mbinddt_type3 : forall (t1 t2 : typ A), mbinddt typ F f (ty_ar t1 t2) = pure F (ty_ar) <⋆> (mbinddt typ F f t1) <⋆> (mbinddt typ F f t2).
+  Proof. reflexivity. Qed.
+
+  Lemma rw_mbinddt_type4 : forall (body : typ A), mbinddt typ F f (ty_univ body) = pure F (ty_univ) <⋆> (mbinddt typ F (fun k => f k ∘ incr [KType]) body).
+  Proof. reflexivity. Qed.
+
+End rw_mbinddt_type.
+
+Hint Rewrite @rw_mbinddt_type1 @rw_mbinddt_type2 @rw_mbinddt_type3 @rw_mbinddt_type4 : sysf_rw.
+
+(** *** <<mfmapdt>> *)
+(******************************************************************************)
+Section rw_mfmapdt_type.
+
+  Context
+    (A B : Type)
+    `{Applicative F}
+    (f : K -> list K * A -> F B).
+
+  Lemma rw_mfmapdt_type1 : forall c, mfmapdt typ F f (ty_c c) = pure F (ty_c c).
+  Proof. reflexivity. Qed.
+
+  Lemma rw_mfmapdt_type2 : forall (a : A), mfmapdt typ F f (ty_v a) = pure F ty_v <⋆> (f KType (nil, a)).
+  Proof.
+    intros. rewrite <- fmap_to_ap.
+    unfold mfmapdt. now rewrite rw_mbinddt_type2.
+  Qed.
+
+  Lemma rw_mfmapdt_type3 : forall (t1 t2 : typ A), mfmapdt typ F f (ty_ar t1 t2) = pure F (ty_ar) <⋆> (mfmapdt typ F f t1) <⋆> (mfmapdt typ F f t2).
+  Proof. reflexivity. Qed.
+
+  Lemma rw_mfmapdt_type4 : forall (body : typ A), mfmapdt typ F f (ty_univ body) = pure F (ty_univ) <⋆> (mfmapdt typ F (fun k => f k ∘ incr [KType]) body).
+  Proof. reflexivity. Qed.
+
+End rw_mfmapdt_type.
+
+Hint Rewrite @rw_mfmapdt_type1 @rw_mfmapdt_type2 @rw_mfmapdt_type3 @rw_mfmapdt_type4 : sysf_rw.
+
+(** *** <<mbindd>> *)
+(******************************************************************************)
+Section rw_mbindd_type.
+
+  Context
+    (A B : Type)
+    (f : forall k, list K * A -> SystemF k B).
+
+  Lemma rw_mbindd_type1 : forall c, mbindd typ f (ty_c c) = ty_c c.
+  Proof. reflexivity. Qed.
+
+  Lemma rw_mbindd_type2 : forall (a : A), mbindd typ f (ty_v a) = f KType (nil, a).
+  Proof. reflexivity. Qed.
+
+  Lemma rw_mbindd_type3 : forall (t1 t2 : typ A), mbindd typ f (ty_ar t1 t2) = ty_ar (mbindd typ f t1) (mbindd typ f t2).
+  Proof. reflexivity. Qed.
+
+  Lemma rw_mbindd_type4 : forall (body : typ A), mbindd typ f (ty_univ body) = ty_univ (mbindd typ (fun k => f k ∘ incr [KType]) body).
+  Proof. reflexivity. Qed.
+
+End rw_mbindd_type.
+
+Hint Rewrite @rw_mbindd_type1 @rw_mbindd_type2 @rw_mbindd_type3 @rw_mbindd_type4 : sysf_rw.
+
+(** *** <<mbind>> *)
+(******************************************************************************)
+Section rw_mbind_type.
+
+  Context
+    (A B : Type)
+    (f : forall k, A -> SystemF k B).
+
+  Lemma rw_mbind_type1 : forall c, mbind typ f (ty_c c) = ty_c c.
+  Proof. reflexivity. Qed.
+
+  Lemma rw_mbind_type2 : forall (a : A), mbind typ f (ty_v a) = f KType a.
+  Proof. reflexivity. Qed.
+
+  Lemma rw_mbind_type3 : forall (t1 t2 : typ A), mbind typ f (ty_ar t1 t2) = ty_ar (mbind typ f t1) (mbind typ f t2).
+  Proof. reflexivity. Qed.
+
+  Lemma rw_mbind_type4 : forall (body : typ A), mbind typ f (ty_univ body) = ty_univ (mbind typ f body).
+  Proof.
+    intros. unfold mbind. rewrite rw_mbindd_type4. repeat fequal. now ext k [w a].
+  Qed.
+
+End rw_mbind_type.
+
+Hint Rewrite @rw_mbind_type1 @rw_mbind_type2 @rw_mbind_type3 @rw_mbind_type4 : sysf_rw.
+
+(** *** <<kbindd>> with <<KType>> *)
+(******************************************************************************)
+Section rw_kbindd_type.
+
+  Context
+    (A : Type)
+    (f : list K * A -> typ A).
+
+  Lemma rw_kbindd_KType_type1 : forall c, kbindd typ KType f (ty_c c) = ty_c c.
+  Proof. reflexivity. Qed.
+
+  Lemma rw_kbindd_KType_type2 : forall a, kbindd typ KType f (ty_v a) = f (nil, a).
+  Proof. reflexivity. Qed.
+
+  Lemma rw_kbindd_KType_type3 : forall (t1 t2 : typ A), kbindd typ KType f (ty_ar t1 t2) = ty_ar (kbindd typ KType f t1) (kbindd typ KType f t2).
+  Proof. reflexivity. Qed.
+
+  Lemma rw_kbindd_KType_type4 : forall (body : typ A), kbindd typ KType f (ty_univ body) = ty_univ (kbindd typ KType (f ∘ incr [KType]) body).
+  Proof.
+    intros. unfold kbindd. simpl_F.
+    do 2 fequal. now ext j [w a].
+  Qed.
+
+End rw_kbindd_type.
+
+Hint Rewrite @rw_kbindd_KType_type1 @rw_kbindd_KType_type2 @rw_kbindd_KType_type3 @rw_kbindd_KType_type4 : sysf_rw.
+
+(** *** <<kbindd>> with <<KTerm>> *)
+(******************************************************************************)
+Section rw_kbindd_type.
+
+  Context
+    (A : Type)
+    (f : list K * A -> term A).
+
+  Lemma rw_kbindd_KTerm_type1 : forall c, kbindd typ KTerm f (ty_c c) = ty_c c.
+  Proof. reflexivity. Qed.
+
+  Lemma rw_kbindd_KTerm_type2 : forall a, kbindd typ KTerm f (ty_v a) = ty_v a.
+  Proof. reflexivity. Qed.
+
+  Lemma rw_kbindd_KTerm_type3 : forall (t1 t2 : typ A), kbindd typ KTerm f (ty_ar t1 t2) = ty_ar (kbindd typ KTerm f t1) (kbindd typ KTerm f t2).
+  Proof. reflexivity. Qed.
+
+  Lemma rw_kbindd_KTerm_type4 : forall (body : typ A), kbindd typ KTerm f (ty_univ body) = ty_univ (kbindd typ KTerm (f ∘ incr [KType]) body).
+  Proof.
+    intros. unfold kbindd. simpl_F.
+    do 2 fequal. now ext j [w a].
+  Qed.
+
+End rw_kbindd_type.
+
+Hint Rewrite @rw_kbindd_KTerm_type1 @rw_kbindd_KTerm_type2 @rw_kbindd_KTerm_type3 @rw_kbindd_KTerm_type4 : sysf_rw.
+
+(** *** <<kbind>> with <<KType>> *)
+(******************************************************************************)
+Section rw_kbind_type.
+
+  Context
+    (A : Type)
+    (f : A -> typ A).
+
+  Lemma rw_kbind_KType_type1 : forall c, kbind typ KType f (ty_c c) = ty_c c.
+  Proof. reflexivity. Qed.
+
+  Lemma rw_kbind_KType_type2 : forall a, kbind typ KType f (ty_v a) = f a.
+  Proof. reflexivity. Qed.
+
+  Lemma rw_kbind_KType_type3 : forall (t1 t2 : typ A), kbind typ KType f (ty_ar t1 t2) = ty_ar (kbind typ KType f t1) (kbind typ KType f t2).
+  Proof. reflexivity. Qed.
+
+  Lemma rw_kbind_KType_type4 : forall (body : typ A), kbind typ KType f (ty_univ body) = ty_univ (kbind typ KType f body).
+  Proof.
+    intros. unfold kbind. now simpl_F.
+  Qed.
+
+End rw_kbind_type.
+
+Hint Rewrite @rw_kbind_KType_type1 @rw_kbind_KType_type2 @rw_kbind_KType_type3 @rw_kbind_KType_type4 : sysf_rw.
+
+(** *** <<kbind>> with <<KTerm>> *)
+(******************************************************************************)
+Section rw_kbind_type.
+
+  Context
+    (A : Type)
+    (f : A -> term A).
+
+  Lemma rw_kbind_KTerm_type1 : forall c, kbind typ KTerm f (ty_c c) = ty_c c.
+  Proof. reflexivity. Qed.
+
+  Lemma rw_kbind_KTerm_type2 : forall a, kbind typ KTerm f (ty_v a) = ty_v a.
+  Proof. reflexivity. Qed.
+
+  Lemma rw_kbind_KTerm_type3 : forall (t1 t2 : typ A), kbind typ KTerm f (ty_ar t1 t2) = ty_ar (kbind typ KTerm f t1) (kbind typ KTerm f t2).
+  Proof. reflexivity. Qed.
+
+  Lemma rw_kbind_KTerm_type4 : forall (body : typ A), kbind typ KTerm f (ty_univ body) = ty_univ (kbind typ KTerm f body).
+  Proof.
+    intros. unfold kbind. now simpl_F.
+  Qed.
+
+End rw_kbind_type.
+
+Hint Rewrite @rw_kbind_KTerm_type1 @rw_kbind_KTerm_type2 @rw_kbind_KTerm_type3 @rw_kbind_KTerm_type4 : sysf_rw.
+
+(** ** List and occurrence operations *)
+(******************************************************************************)
+
+(** *** <<tomlistd>> *)
+(******************************************************************************)
+Section rw_tomlistd_type.
+
+  Context
+    (A : Type).
+
+  Lemma rw_tomlistd_type1 : forall c, tomlistd (A := A) typ (ty_c c) = nil.
+  Proof. reflexivity. Qed.
+
+  Lemma rw_tomlistd_type2 : forall (a : A), tomlistd typ (ty_v a) = [ (nil, (KType, a)) ].
+  Proof. reflexivity. Qed.
+
+  Lemma rw_tomlistd_type3 : forall (t1 t2 : typ A), tomlistd typ (ty_ar t1 t2) = tomlistd typ t1 ++ tomlistd typ t2.
+  Proof. reflexivity. Qed.
+
+  Lemma rw_tomlistd_type4 : forall (body : typ A), tomlistd typ (ty_univ body) = fmap list (incr [KType]) (tomlistd typ body).
+  Proof.
+    intros. unfold tomlistd, tomlistd_gen.
+    rewrite rw_mfmapdt_type4. cbn.
+    compose near body on right. unfold mfmapdt.
+    rewrite (dtp_mbinddt_morphism
+               (list (@K I2)) typ SystemF (const (list _)) (const (list _)) (ϕ := (fun _ => fmap list (incr [KType])))
+               (fun (k : @K I2) => fmap (const (list (list K2 * (K2 * A)))) (mret SystemF k) ∘ (fun '(w, a) => [(w, (k, a))]))).
+    fequal. now ext k [w a].
+  Qed.
+
+End rw_tomlistd_type.
+
+Hint Rewrite @rw_tomlistd_type1 @rw_tomlistd_type2 @rw_tomlistd_type3 @rw_tomlistd_type4 : sysf_rw.
+
+(** *** <<toklistd>> with <<KType>> *)
+(******************************************************************************)
+Section rw_toklistd_KType_type.
+
+  Context
+    (A : Type).
+
+  Lemma rw_toklistd_KType_type1 : forall c, toklistd (A := A) typ KType (ty_c c) = nil.
+  Proof. reflexivity. Qed.
+
+  Lemma rw_toklistd_KType_type2 : forall (a : A), toklistd typ KType (ty_v a) = [ (nil, a) ].
+  Proof. reflexivity. Qed.
+
+  Lemma rw_toklistd_KType_type3 : forall (t1 t2 : typ A), toklistd typ KType (ty_ar t1 t2) = toklistd typ KType t1 ++ toklistd typ KType t2.
+  Proof. intros. unfold toklistd, compose. rewrite rw_tomlistd_type3. now autorewrite with tea_list. Qed.
+
+  Lemma rw_toklistd_KType_type4 : forall (body : typ A), toklistd typ KType (ty_univ body) = fmap list (incr [KType]) (toklistd typ KType body).
+  Proof. intros. unfold toklistd, compose. rewrite rw_tomlistd_type4.
+         induction (tomlistd typ body).
+         - reflexivity.
+         - destruct a as [w [k a]]. compare values k and KType.
+           + cbn. now rewrite <- IHl.
+           + repeat (autorewrite with tea_list; auto).
+             rewrite <- IHl.
+             change (incr [KType] (w, (k, a))) with (KType :: w, (k, a)).
+             rewrite filterk_cons_neq; auto.
+  Qed.
+
+End rw_toklistd_KType_type.
+
+Hint Rewrite @rw_toklistd_KType_type1 @rw_toklistd_KType_type2 @rw_toklistd_KType_type3 @rw_toklistd_KType_type4 : sysf_rw.
+
+(** *** <<toklistd>> with <<KTerm>> *)
+(******************************************************************************)
+Section rw_toklistd_KTerm_type.
+
+  Context
+    (A : Type).
+
+  Lemma rw_toklistd_KTerm_type1 : forall c, toklistd (A := A) typ KTerm (ty_c c) = nil.
+  Proof. reflexivity. Qed.
+
+  Lemma rw_toklistd_KTerm_type2 : forall (a : A), toklistd typ KTerm (ty_v a) = nil.
+  Proof. reflexivity. Qed.
+
+  Lemma rw_toklistd_KTerm_type3 : forall (t1 t2 : typ A), toklistd typ KTerm (ty_ar t1 t2) = toklistd typ KTerm t1 ++ toklistd typ KTerm t2.
+  Proof. intros. unfold toklistd, compose. rewrite rw_tomlistd_type3. now autorewrite with tea_list. Qed.
+
+  Lemma rw_toklistd_KTerm_type4 : forall (body : typ A), toklistd typ KTerm (ty_univ body) = fmap list (incr [KType]) (toklistd typ KTerm body).
+  Proof.
+    intros. unfold toklistd, compose. rewrite rw_tomlistd_type4.
+    induction (tomlistd typ body).
+    - reflexivity.
+    - destruct a as [w [k a]]. compare values k and KTerm.
+      + cbn. now rewrite <- IHl.
+      + repeat (autorewrite with tea_list; auto).
+        rewrite <- IHl.
+        change (incr [KType] (w, (k, a))) with (KType :: w, (k, a)).
+        rewrite filterk_cons_neq; auto.
+  Qed.
+
+End rw_toklistd_KTerm_type.
+
+Hint Rewrite @rw_toklistd_KTerm_type1 @rw_toklistd_KTerm_type2 @rw_toklistd_KTerm_type3 @rw_toklistd_KTerm_type4 : sysf_rw.
+
+Corollary rw_toklistd_KTerm_type : forall A (τ : typ A), toklistd typ KTerm τ = nil.
+Proof.
+  intros. induction τ; autorewrite with sysf_rw.
+  - trivial.
+  - trivial.
+  - now rewrite IHτ1, IHτ2.
+  - now rewrite IHτ.
+Qed.
+
+(** *** <<tomlist>> *)
+(******************************************************************************)
+Section rw_tomlist_type.
+
+  Context
+    (A : Type).
+
+  Lemma rw_tomlist_type1 : forall c, tomlist (A := A) typ (ty_c c) = nil.
+  Proof. reflexivity. Qed.
+
+  Lemma rw_tomlist_type2 : forall (a : A), tomlist typ (ty_v a) = [ (KType, a) ].
+  Proof. reflexivity. Qed.
+
+  Lemma rw_tomlist_type3 : forall (t1 t2 : typ A), tomlist typ (ty_ar t1 t2) = tomlist typ t1 ++ tomlist typ t2.
+  Proof. intros. unfold tomlist, compose. rewrite rw_tomlistd_type3. now autorewrite with tea_list. Qed.
+
+  Lemma rw_tomlist_type4 : forall (body : typ A), tomlist typ (ty_univ body) = (tomlist typ body).
+  Proof. intros. unfold tomlist, compose. rewrite rw_tomlistd_type4.
+         compose near (tomlistd typ body) on left. rewrite (fun_fmap_fmap list).
+         fequal. now ext [w a].
+  Qed.
+
+End rw_tomlist_type.
+
+Hint Rewrite @rw_tomlist_type1 @rw_tomlist_type2 @rw_tomlist_type3 @rw_tomlist_type4 : sysf_rw.
+
+(** *** <<toklist>> with <<KType>> *)
+(******************************************************************************)
+Section rw_toklist_KType_type.
+
+  Context
+    (A : Type).
+
+  Lemma rw_toklist_KType_type1 : forall c, toklist (A := A) typ KType (ty_c c) = nil.
+  Proof. reflexivity. Qed.
+
+  Lemma rw_toklist_KType_type2 : forall (a : A), toklist typ KType (ty_v a) = [ a ].
+  Proof. reflexivity. Qed.
+
+  Lemma rw_toklist_KType_type3 : forall (t1 t2 : typ A), toklist typ KType (ty_ar t1 t2) = toklist typ KType t1 ++ toklist typ KType t2.
+  Proof. intros. unfold toklist, compose. rewrite rw_toklistd_KType_type3. now autorewrite with tea_list. Qed.
+
+  Lemma rw_toklist_KType_type4 : forall (body : typ A), toklist typ KType (ty_univ body) = (toklist typ KType body).
+  Proof. intros. unfold toklist, compose. rewrite rw_toklistd_KType_type4.
+         compose near (toklistd typ KType body) on left. rewrite (fun_fmap_fmap list).
+         fequal. now ext [w a]. Qed.
+
+End rw_toklist_KType_type.
+
+Hint Rewrite @rw_toklist_KType_type1 @rw_toklist_KType_type2 @rw_toklist_KType_type3 @rw_toklist_KType_type4 : sysf_rw.
+
+(** *** <<toklist>> with <<KTerm>> *)
+(******************************************************************************)
+Section rw_toklist_KTerm_type.
+
+  Context
+    (A : Type).
+
+  Lemma rw_toklist_KTerm_type1 : forall c, toklist (A := A) typ KTerm (ty_c c) = nil.
+  Proof. reflexivity. Qed.
+
+  Lemma rw_toklist_KTerm_type2 : forall (a : A), toklist typ KTerm (ty_v a) = nil.
+  Proof. reflexivity. Qed.
+
+  Lemma rw_toklist_KTerm_type3 : forall (t1 t2 : typ A), toklist typ KTerm (ty_ar t1 t2) = toklist typ KTerm t1 ++ toklist typ KTerm t2.
+  Proof. intros. unfold toklist, compose. rewrite rw_toklistd_KTerm_type3. now autorewrite with tea_list. Qed.
+
+  Lemma rw_toklist_KTerm_type4 : forall (body : typ A), toklist typ KTerm (ty_univ body) = (toklist typ KTerm body).
+  Proof. intros. unfold toklist, compose. rewrite rw_toklistd_KTerm_type4.
+         compose near (toklistd typ KTerm body) on left. rewrite (fun_fmap_fmap list).
+         fequal. now ext [w a]. Qed.
+
+End rw_toklist_KTerm_type.
+
+Hint Rewrite @rw_toklist_KTerm_type1 @rw_toklist_KTerm_type2 @rw_toklist_KTerm_type3 @rw_toklist_KTerm_type4 : sysf_rw.
+
+Corollary rw_toklist_KTerm_type : forall A (τ : typ A), toklist typ KTerm τ = nil.
+Proof.
+  intros. induction τ; autorewrite with sysf_rw.
+  - trivial.
+  - trivial.
+  - now rewrite IHτ1, IHτ2.
+  - now rewrite IHτ.
+Qed.
+
+(** *** Variable occurrence with context *)
+(******************************************************************************)
+Section rw_tomsetd_type.
+
+  Context
+    (A : Type)
+    (k : K2).
+
+  Implicit Types
+           (w : list K) (a : A).
+
+  Lemma rw_tomsetd_type1 : forall c w a, (w, (k, a)) ∈md (ty_c c) <-> False.
+  Proof.
+    intros. unfold tomsetd, compose. autorewrite with sysf_rw. easy.
+  Qed.
+
+  Lemma rw_tomsetd_type2 : forall w a a', (w, (k, a)) ∈md (ty_v a') <-> w = nil /\ k = KType /\ a = a'.
+  Proof.
+    intros. unfold tomsetd, compose. autorewrite with sysf_rw tea_list.
+    splits.
+    - now inversion 1.
+    - firstorder. now subst.
+  Qed.
+
+  Lemma rw_tomsetd_type3 : forall w a (t1 t2 : typ A), (w, (k, a)) ∈md ty_ar t1 t2 <-> ((w, (k, a)) ∈md t1 \/ (w, (k, a)) ∈md t2).
+  Proof.
+    intros. unfold tomsetd, compose.
+    now autorewrite with sysf_rw tea_list tea_set.
+  Qed.
+
+  Lemma rw_tomsetd_type4 : forall w a (body : typ A), (w, (k, a)) ∈md (ty_univ body) <-> exists w', (w', (k, a)) ∈md body /\ w = (cons KType w').
+  Proof.
+    intros. unfold tomsetd, compose. autorewrite with sysf_rw.
+    rewrite (in_fmap_iff list). splits.
+    - intros [[w'' [j a']] [rest1 rest2]]. cbn in *. inverts rest2. eauto.
+    - intros [w' rest]. exists (w', (k, a)). now inverts rest.
+  Qed.
+
+End rw_tomsetd_type.
+
+Hint Rewrite @rw_tomsetd_type1 @rw_tomsetd_type2 @rw_tomsetd_type3 @rw_tomsetd_type4 : sysf_rw.
+
+Corollary rw_tomsetd_type_KTerm : forall w A a (τ : typ A), (w, (KTerm, a)) ∈md τ <-> False.
+Proof.
+  intros. generalize dependent w.
+  induction τ; intro w; autorewrite with sysf_rw; try easy.
+  - rewrite IHτ1, IHτ2. tauto.
+  - split; try tauto.
+    intros [w' [rest1 rest2]]. now rewrite IHτ in rest1.
+Qed.
+
+(** *** Variable occurrence without context *)
+(******************************************************************************)
+Section rw_tomset_type.
+
+  Context
+    (A : Type)
+    (k : K2).
+
+  Implicit Types (a : A).
+
+  Lemma rw_tomset_type1 : forall c a, (k, a) ∈m (ty_c c) <-> False.
+  Proof. intros. rewrite ind_iff_in. firstorder eauto. Qed.
+
+  Lemma rw_tomset_type2 : forall a a', (k, a) ∈m (ty_v a') <-> k = KType /\ a = a'.
+  Proof. intros. rewrite ind_iff_in. setoid_rewrite rw_tomsetd_type2. firstorder eauto.  Qed.
+
+  Lemma rw_tomset_type3 : forall a (t1 t2 : typ A), (k, a) ∈m ty_ar t1 t2 <-> (k, a) ∈m t1 \/ (k, a) ∈m t2.
+  Proof. intros. repeat rewrite ind_iff_in. setoid_rewrite rw_tomsetd_type3. firstorder eauto. Qed.
+
+  Lemma rw_tomset_type4 : forall a (body : typ A), (k, a) ∈m (ty_univ body) <-> (k, a) ∈m body.
+  Proof. intros. repeat rewrite ind_iff_in. setoid_rewrite rw_tomsetd_type4. firstorder eauto.  Qed.
+
+End rw_tomset_type.
+
+Hint Rewrite @rw_tomset_type1 @rw_tomset_type2 @rw_tomset_type3 @rw_tomset_type4 : sysf_rw.
+
+(** ** <<free>> and <<freeset>> *)
+(******************************************************************************)
+
+(** *** <<free>> with <<KType>> *)
+(******************************************************************************)
+Section rw_free_KType_type.
+
+  Lemma rw_free_KType_type11 : forall (x : atom), free typ KType (ty_v (Fr x)) = [x].
+  Proof.
+    reflexivity.
+  Qed.
+
+  Lemma rw_free_KType_type12 : forall (n : nat), free typ KType (ty_v (Bd n)) = [].
+  Proof.
+    reflexivity.
+  Qed.
+
+  Lemma rw_free_KType_type2 : forall (c : base_typ), free typ KType (ty_c c) = [].
+  Proof.
+    reflexivity.
+  Qed.
+
+  Lemma rw_free_KType_type3 : forall t1 t2, free typ KType (ty_ar t1 t2) = free typ KType t1 ++ free typ KType t2.
+  Proof.
+    intros. unfold free. now autorewrite with sysf_rw tea_list.
+  Qed.
+
+  Lemma rw_free_KType_type4 : forall t, free typ KType (ty_univ t) = free typ KType t.
+  Proof.
+    intros. unfold free. now autorewrite with sysf_rw tea_list.
+  Qed.
+
+End rw_free_KType_type.
+
+Hint Rewrite rw_free_KType_type11 rw_free_KType_type12 rw_free_KType_type2 rw_free_KType_type3 rw_free_KType_type4 : sysf_rw.
+
+(** *** <<freeset>> with <<KType>> *)
+(******************************************************************************)
+Section rw_freeset_KType_type.
+
+  Lemma rw_freeset_KType_type11 : forall (x : atom), freeset typ KType (ty_v (Fr x)) [=] {{ x }}.
+  Proof.
+    unfold freeset. intros. autorewrite with sysf_rw tea_rw_atoms. fsetdec.
+  Qed.
+
+  Lemma rw_freeset_KType_type12 : forall (n : nat), freeset typ KType (ty_v (Bd n)) [=] ∅.
+  Proof.
+    reflexivity.
+  Qed.
+
+  Lemma rw_freeset_KType_type2 : forall (c : base_typ), freeset typ KType (ty_c c) [=] ∅.
+  Proof.
+    reflexivity.
+  Qed.
+
+  Lemma rw_freeset_KType_type3 : forall t1 t2, freeset typ KType (ty_ar t1 t2) [=] freeset typ KType t1 ∪ freeset typ KType t2.
+  Proof.
+    intros. unfold freeset. autorewrite with sysf_rw tea_rw_atoms. reflexivity.
+  Qed.
+
+  Lemma rw_freeset_KType_type4 : forall t, freeset typ KType (ty_univ t) [=] freeset typ KType t.
+  Proof.
+    intros. unfold freeset. autorewrite with sysf_rw tea_rw_atoms. reflexivity.
+  Qed.
+
+End rw_freeset_KType_type.
+
+Hint Rewrite rw_freeset_KType_type11 rw_freeset_KType_type12 rw_freeset_KType_type2 rw_freeset_KType_type3 rw_freeset_KType_type4 : sysf_rw.
+
+(** *** <<free>> with <<KTerm>> *)
+(******************************************************************************)
+Section rw_free_KTerm_type.
+
+  Lemma rw_free_KTerm_type11 : forall (x : atom), free typ KTerm (ty_v (Fr x)) = [].
+  Proof.
+    reflexivity.
+  Qed.
+
+  Lemma rw_free_KTerm_type12 : forall (n : nat), free typ KTerm (ty_v (Bd n)) = [].
+  Proof.
+    reflexivity.
+  Qed.
+
+  Lemma rw_free_KTerm_type2 : forall (c : base_typ), free typ KTerm (ty_c c) = [].
+  Proof.
+    reflexivity.
+  Qed.
+
+  Lemma rw_free_KTerm_type3 : forall t1 t2, free typ KTerm (ty_ar t1 t2) = free typ KTerm t1 ++ free typ KTerm t2.
+  Proof. intros. unfold free. now autorewrite with sysf_rw tea_list. Qed.
+
+  Lemma rw_free_KTerm_type4 : forall t, free typ KTerm (ty_univ t) = free typ KTerm t.
+  Proof. intros. unfold free. now autorewrite with sysf_rw tea_list. Qed.
+
+End rw_free_KTerm_type.
+
+Hint Rewrite rw_free_KTerm_type11 rw_free_KTerm_type12 rw_free_KTerm_type2 rw_free_KTerm_type3 rw_free_KTerm_type4 : sysf_rw.
+
+Corollary rw_free_KTerm_type : forall (τ : typ leaf), free typ KTerm τ = [].
+Proof.
+  intros. induction τ; autorewrite with sysf_rw.
+  - trivial.
+  - trivial.
+  - now rewrite IHτ1, IHτ2.
+  - now rewrite IHτ.
+Qed.
+
+(** *** <<freeset>> with <<KTerm>> *)
+(******************************************************************************)
+Section rw_freeset_KTerm_type.
+
+  Lemma rw_freeset_KTerm_type11 : forall (x : atom), freeset typ KTerm (ty_v (Fr x)) [=] ∅.
+  Proof.
+    unfold freeset. intros. rewrite rw_free_KTerm_type11. autorewrite with tea_rw_atoms. fsetdec. Qed.
+
+  Lemma rw_freeset_KTerm_type12 : forall (n : nat), freeset typ KTerm (ty_v (Bd n)) [=] ∅.
+  Proof.
+    reflexivity.
+  Qed.
+
+  Lemma rw_freeset_KTerm_type2 : forall (c : base_typ), freeset typ KTerm (ty_c c) [=] ∅.
+  Proof.
+    reflexivity.
+  Qed.
+
+  Lemma rw_freeset_KTerm_type3 : forall t1 t2, freeset typ KTerm (ty_ar t1 t2) [=] freeset typ KTerm t1 ∪ freeset typ KTerm t2.
+  Proof.
+    intros. unfold freeset. autorewrite with sysf_rw tea_rw_atoms. reflexivity.
+  Qed.
+
+  Lemma rw_freeset_KTerm_type4 : forall t, freeset typ KTerm (ty_univ t) [=] freeset typ KTerm t.
+  Proof.
+    intros. unfold freeset. autorewrite with sysf_rw tea_rw_atoms. reflexivity.
+  Qed.
+
+End rw_freeset_KTerm_type.
+
+Hint Rewrite rw_freeset_KTerm_type11 rw_freeset_KTerm_type12 rw_freeset_KTerm_type2 rw_freeset_KTerm_type3 rw_freeset_KTerm_type4 : sysf_rw.
+
+Corollary rw_freeset_KTerm_type : forall (τ : typ leaf), freeset typ KTerm τ [=] ∅.
+Proof.
+  intros. induction τ.
+  - autorewrite with sysf_rw. fsetdec.
+  - cbn. fsetdec.
+  - autorewrite with sysf_rw. fsetdec.
+  - autorewrite with sysf_rw. fsetdec.
+Qed.
+
+Hint Rewrite rw_freeset_KTerm_type : sysf_rw.
+
+(** ** Locally nameless operations *)
+(******************************************************************************)
+
+(** *** <<open>> *)
+(******************************************************************************)
+Section rw_open_type.
+
+  Context
+    (u : typ leaf).
+
+  Lemma rw_open_type1 : forall c, open typ KType u (ty_c c) = ty_c c.
+  Proof. reflexivity. Qed.
+
+  Lemma rw_open_type2 : forall (l : leaf), open typ KType u (ty_v l) = open_loc KType u (nil, l).
+  Proof. reflexivity. Qed.
+
+  Lemma rw_open_type3 : forall (t1 t2 : typ leaf), open typ KType u (ty_ar t1 t2) = ty_ar (open typ KType u t1) (open typ KType u t2).
+  Proof. reflexivity. Qed.
+
+End rw_open_type.
+
+Hint Rewrite @rw_open_type1 @rw_open_type2 @rw_open_type3 : sysf_rw.
+
+(** *** <<subst>> *)
+(******************************************************************************)
+Section rw_subst_type.
+
+  Context
+    (x : atom)
+    (u : typ leaf).
+
+  Lemma rw_subst_type1 : forall c, subst typ KType x u (ty_c c) = ty_c c.
+  Proof. reflexivity. Qed.
+
+  Lemma rw_subst_type2 : forall (l : leaf), subst typ KType x u (ty_v l) = subst_loc KType x u l.
+  Proof. reflexivity. Qed.
+
+  Lemma rw_subst_type3 : forall (t1 t2 : typ leaf), subst typ KType x u (ty_ar t1 t2) = ty_ar (subst typ KType x u t1) (subst typ KType x u t2).
+  Proof. reflexivity. Qed.
+
+  Lemma rw_subst_type4 : forall (t : typ leaf), subst typ KType x u (ty_univ t) = ty_univ (subst typ KType x u t).
+  Proof.
+    intros. unfold subst. now autorewrite with sysf_rw.
+  Qed.
+
+End rw_subst_type.
+
+Hint Rewrite @rw_subst_type1 @rw_subst_type2 @rw_subst_type3 @rw_subst_type4 : sysf_rw.
+
+(** *** <<locally_closed>> with <<KType>> *)
+(******************************************************************************)
+Section rw_lc_KType_type.
+
+  Lemma rw_lc_KType_type1 : forall c, locally_closed typ KType (ty_c c).
+  Proof.
+    intros. unfold locally_closed, locally_closed_gap; introv hyp.
+    now rewrite rw_tomsetd_type1 in hyp.
+  Qed.
+
+  Lemma rw_lc_KType_type2 : forall (l : leaf), locally_closed typ KType (ty_v l) <-> exists x, l = Fr x.
+  Proof.
+    intros. unfold locally_closed, locally_closed_gap.
+    setoid_rewrite rw_tomsetd_type2. split.
+    - introv hyp. destruct l.
+      + eauto.
+      + enough (n < 0). lia. now apply (hyp [] (Bd n)).
+    - intros [x heq]. subst. introv hyp. inversion hyp.
+      inverts H0. cbn; trivial.
+  Qed.
+
+  Lemma rw_lc_KType_type3 : forall (t1 t2 : typ leaf), locally_closed typ KType (ty_ar t1 t2) <-> (locally_closed typ KType t1 /\ locally_closed typ KType t2).
+  Proof.
+    intros. unfold locally_closed, locally_closed_gap.
+    setoid_rewrite rw_tomsetd_type3. firstorder.
+  Qed.
+
+  #[local] Open Scope nat_scope.
+
+  Lemma rw_lc_KType_type4 : forall (t : typ leaf), locally_closed typ KType (ty_univ t) <-> locally_closed_gap typ KType 1 t.
+  Proof.
+    intros. unfold locally_closed, locally_closed_gap.
+    setoid_rewrite rw_tomsetd_type4. split.
+    - intros hyp w l Hin.
+      specialize (hyp (KType :: w) l). cbn in *.
+      assert (rw : S (countk (@KType : K) w + 0) = (countk KType w + 1)) by lia.
+      rewrite <- rw. apply hyp. eauto.
+    - intros hyp w l [w' [H1 H2]]. subst.
+      specialize (hyp w' l H1). cbn in *. destruct l.
+      + easy.
+      + lia.
+  Qed.
+
+End rw_lc_KType_type.
+
+Hint Rewrite @rw_lc_KType_type1 @rw_lc_KType_type2 @rw_lc_KType_type3 @rw_lc_KType_type4 : sysf_rw.
+
+(** *** <<locally_closed>> with <<KTerm>> *)
+(******************************************************************************)
+Section rw_lc_KTerm_type.
+
+  Lemma rw_lc_KTerm_type : forall τ, locally_closed typ KTerm τ.
+  Proof.
+    intros. unfold locally_closed, locally_closed_gap.
+    intros. now rewrite rw_tomsetd_type_KTerm in H.
+  Qed.
+
+End rw_lc_KTerm_type.
+
+Hint Rewrite @rw_lc_KTerm_type : sysf_rw.
+
+(** *** <<locally_closed>> with <<KTerm>> *)
+(******************************************************************************)
+Section rw_scoped_KTerm_type.
+
+  Lemma rw_scoped_KTerm_type : forall τ (vars : AtomSet.t), scoped typ KTerm τ vars.
+  Proof.
+    intros. unfold scoped. autorewrite with sysf_rw. fsetdec.
+  Qed.
+
+End rw_scoped_KTerm_type.
+
+(** * Rewriting principles for <<ok_type>> *)
+(******************************************************************************)
+Lemma ok_type_ar : forall Δ τ1 τ2,
+    ok_type Δ (ty_ar τ1 τ2) <->
+    ok_type Δ τ1 /\ ok_type Δ τ2.
+Proof.
+  intros. unfold ok_type.
+  unfold scoped.
+  autorewrite with sysf_rw.
+  intuition fsetdec.
+Qed.
+
+Lemma ok_type_univ : forall Δ τ,
+    ok_type Δ (ty_univ τ) <->
+    scoped typ KType τ (domset Δ) /\
+    locally_closed_gap typ KType 1 τ.
+Proof.
+  intros. unfold ok_type.
+  unfold scoped.
+  now autorewrite with sysf_rw.
+Qed.
+
+(** * Rewriting principles for <<ok_term>> *)
+(******************************************************************************)
+Lemma ok_term_abs : forall Δ Γ τ t,
+    ok_term Δ Γ (tm_abs τ t) <->
+    ok_type Δ τ /\
+    scoped term KTerm t (domset Γ) /\
+    scoped term KType t (domset Δ) /\
+    locally_closed term KType t /\
+    locally_closed_gap term KTerm 1 t.
+Proof.
+  intros. unfold ok_type, ok_term.
+  unfold scoped.
+  repeat autorewrite with sysf_rw.
+  (*
+  rewrite rw_freeset_KTerm_type.
+  intuition fsetdec.
+*)
+Admitted.
+
+Lemma ok_term_app : forall Δ Γ t1 t2,
+    ok_term Δ Γ (tm_app t1 t2) <-> ok_term Δ Γ t1 /\ ok_term Δ Γ t2.
+Proof.
+  intros. unfold ok_term, scoped.
+  (*
+  simpl_F. intuition fsetdec.
+   *)
+Admitted.
