SystemF/Theory.v
@@ -1,0 +1,549 @@
+From Tealeaves Require Import
+     Functors.List
+     LN.Leaf LN.Atom LN.AtomSet LN.AssocList
+     LN.Multisorted.Operations
+     LN.Multisorted.Theory.
+
+From Multisorted Require Import
+     Classes.DTM
+     Theory.DTMContainer.
+
+From Coq Require Import
+     Sorting.Permutation.
+
+From Tealeaves.Examples Require Import
+     SystemF.Language
+     SystemF.Rewriting
+     SystemF.Contexts.
+
+Implicit Types (x : atom).
+
+Import SetlikeFunctor.Notations.
+Import DTMContainer.Notations.
+Import List.ListNotations.
+Import LN.AssocList.Notations.
+
+(** * Odds and Ends *)
+(******************************************************************************)
+Lemma permutation_fact : forall A (l1 l2 l3 : list A),
+    Permutation ((l1 ++ l2) ++ l3)
+                ((l1 ++ l3) ++ l2).
+Proof.
+  intros. simpl_alist. apply Permutation_app. auto.
+  apply Permutation_app_comm.
+Qed.
+
+Lemma rw_subst_type13 {x y} {τ'} :
+  x <> y ->
+  subst typ KType x τ' (ty_v (Fr y)) = ty_v (Fr y).
+Proof.
+  autorewrite with sysf_rw. cbn. compare values x and y.
+Qed.
+
+(** * Properties of the typing judgment <<Δ ; Γ ⊢ t : τ>> *)
+(******************************************************************************)
+
+(** ** Structural properties <<Δ ; Γ ⊢ t : τ>> in <<Δ>> *)
+(******************************************************************************)
+
+(** *** <<Δ>> is always well-formed *)
+(******************************************************************************)
+Lemma j_kind_ctx_wf : forall Δ Γ t τ,
+    (Δ ; Γ ⊢ t : τ) ->
+    ok_kind_ctx Δ.
+Proof.
+  unfold ok_kind_ctx; induction 1; cleanup_cofinite.
+  all: (autorewrite with tea_rw_uniq in *; intuition).
+Qed.
+
+(** *** Permutation *)
+(******************************************************************************)
+Theorem j_kind_ctx_perm : forall Δ1 Δ2 Γ t τ,
+    Permutation Δ1 Δ2 ->
+    (Δ1 ; Γ ⊢ t : τ) ->
+    (Δ2 ; Γ ⊢ t : τ).
+Proof.
+  introv perm j. generalize dependent Δ2.
+  induction j; introv Hperm.
+  - eauto using Judgment, Permutation_sym with sysf_ctx.
+  - eauto using Judgment.
+  - eauto using Judgment.
+  - eapply j_univ.
+    eauto using Permutation_app_tail.
+  - eauto using Judgment, ok_type_perm1.
+Qed.
+
+Corollary j_kind_ctx_perm1 : forall Δ1 Δ2 x Γ t τ,
+    ((Δ1 ++ x ~ tt) ++ Δ2 ; Γ ⊢ t : τ) ->
+    ((Δ1 ++ Δ2) ++ x ~ tt ; Γ ⊢ t : τ).
+Proof.
+  eauto using j_kind_ctx_perm, permutation_fact.
+Qed.
+
+Hint Resolve ok_kind_ctx_app1 : sysf_ctx.
+
+(** *** Weakening *)
+(******************************************************************************)
+Theorem weak_j_kind_ctx : forall Δ1 Δ2 Γ t τ,
+    ok_kind_ctx Δ2 ->
+    disjoint Δ1 Δ2 ->
+    (Δ1 ; Γ ⊢ t : τ) ->
+    (Δ1 ++ Δ2 ; Γ ⊢ t : τ).
+Proof.
+  introv ok disj j. induction j.
+  - apply j_var; auto with sysf_ctx.
+  - apply j_abs with (L := L); auto with sysf_ctx.
+  - apply j_app with (τ1 := τ1); auto.
+  - rename H0 into IH.
+    apply j_univ with (L := L ∪ domset Δ2).
+    intros_cof IH. apply j_kind_ctx_perm1.
+    autorewrite with tea_rw_disj in *.
+    intuition fsetdec.
+  - apply j_inst; auto with sysf_ctx.
+Qed.
+
+
+Lemma rw_subst_term_var {x y} {τ} :
+  x <> y ->
+  subst term KType x τ (tm_var (Fr y)) = tm_var (Fr y).
+Proof.
+  autorewrite with sysf_rw. cbn. compare values x and y.
+Qed.
+
+(** *** Substitution *)
+(******************************************************************************)
+Theorem subst_j_kind_ctx : forall Δ1 x Δ2 Γ t τ τ',
+    ok_type (Δ1 ++ Δ2) τ' ->
+    (Δ1 ++ x ~ tt ++ Δ2 ; Γ ⊢ t : τ) ->
+    (Δ1 ++ Δ2 ; envmap (subst typ KType x τ') Γ ⊢ subst term KType x τ' t : subst typ KType x τ' τ).
+Proof.
+  introv Hok j. remember (Δ1 ++ x ~ tt ++ Δ2) as rem.
+  generalize dependent Δ2. induction j; intros; subst.
+  - cbn. constructor.
+    + eauto with sysf_ctx.
+    + apply ok_type_ctx_sub.
+      * eauto.
+      * eauto.
+      * eapply ok_type_lc; eauto.
+    + rewrite in_envmap_iff. eauto.
+  - rename H0 into IH. simpl_F.
+    assert (rw : subst term (KType : K) x τ' (tm_abs τ1 t) =
+                 (tm_abs (subst typ KType x τ' τ1) (subst term (KType : K) x τ' t))) by admit.
+    rewrite rw. clear rw.
+    apply j_abs with (L := L ∪ {{ x }}).
+    intros_cof IH.
+    rewrite (subst_open_neq term) in IH
+      by (discriminate + apply rw_lc_KTerm_type).
+    rewrite rw_subst_term_var in IH; [ |fsetdec].
+    rewrite envmap_app in IH. auto.
+  - assert (rw : subst term KType x τ' (tm_app t1 t2) =
+                 tm_app (subst term KType x τ' t1) (subst term KType x τ' t2)) by admit.
+    rewrite rw; clear rw.
+    eapply j_app.
+    + autorewrite with sysf_rw in IHj1; eauto.
+    + eauto.
+  - rename H0 into IH. simpl_F.
+    assert (rw : subst term KType x τ' (tm_tab t) =
+                 tm_tab (subst term KType x τ' t)) by admit.
+    rewrite rw; clear rw.
+    apply j_univ with (L := L ∪ {{x}}).
+    intros_cof IH. simpl_alist in *.
+    assert (x <> e) by fsetdec.
+    rewrite (subst_open_eq term) in IH.
+    2:{ now inverts Hok. }
+    rewrite (subst_open_eq typ) in IH.
+    2:{ now inverts Hok. }
+    rewrite rw_subst_type13 in IH; auto.
+    apply IH.
+    + change_alist ((Δ1 ++ Δ2) ++ e ~ tt).
+      auto using ok_type_weak_r.
+    + reflexivity.
+  - simpl_F. rewrite (subst_open_eq typ); auto.
+    2:{ clear IHj j. eapply ok_type_lc; eauto. }
+    apply j_inst; auto with sysf_ctx.
+Admitted.
+
+(** ** Properties of <<Δ ; Γ ⊢ t : τ>> in <<Γ>> *)
+(******************************************************************************)
+
+(** *** <<Γ>> is always well-formed *)
+(******************************************************************************)
+Lemma j_type_ctx_wf : forall Δ Γ t τ,
+    (Δ ; Γ ⊢ t : τ) ->
+    ok_type_ctx Δ Γ.
+Proof.
+  introv j. induction j; try assumption.
+  - cleanup_cofinite. eauto using ok_type_ctx_inv_app_l.
+  - rename H0 into IH.
+    pick fresh e for L.
+    (*
+    pick fresh e for (L ∪ concatAtoms (envmap (freeset typ KType) Γ)).
+     *)
+    specialize_cof IH e.
+    apply (ok_type_ctx_stren1) with (x := e).
+    + assumption.
+    + admit.
+Admitted.
+
+(** *** Tactical corollaries *)
+(******************************************************************************)
+Corollary j_type_ctx1 : forall Δ Γ t τ x τ2,
+    (Δ ; Γ ⊢ t : τ) ->
+    (x, τ2) ∈ Γ ->
+    ok_type Δ τ2.
+Proof.
+  eauto using ok_type_ctx_binds, j_type_ctx_wf.
+Qed.
+
+Corollary j_type_ctx2 : forall Δ Γ t τ1 τ2 x,
+    (Δ ; Γ ++ x ~ τ2 ⊢ t : τ1) ->
+    ok_type Δ τ2.
+Proof.
+  intros. eapply j_type_ctx1. eauto.
+  autorewrite with tea_list. eauto.
+Qed.
+
+(** *** Permutation *)
+(******************************************************************************)
+Theorem perm_j_type_ctx : forall Δ Γ1 Γ2 t τ,
+    (Δ ; Γ1 ⊢ t : τ) ->
+    Permutation Γ1 Γ2 ->
+    (Δ ; Γ2 ⊢ t : τ).
+Proof.
+  introv j perm. generalize dependent Γ2.
+  induction j; intros ? Hperm; try eauto using Judgment.
+  - constructor.
+    + eauto using ok_kind_ctx_perm.
+    + rewrite ok_type_ctx_perm_gamma;
+        eauto using Permutation_sym.
+    + symmetry in Hperm. erewrite List.perm_set_eq; eauto.
+  - econstructor; eauto using Permutation_app_tail.
+Qed.
+
+Corollary perm_j_type_ctx_iff : forall Δ Γ1 Γ2 t τ,
+    Permutation Γ1 Γ2 ->
+    (Δ ; Γ1 ⊢ t : τ) <->
+    (Δ ; Γ2 ⊢ t : τ).
+Proof.
+  introv Hperm. assert (Permutation Γ2 Γ1) by now symmetry.
+  split; eauto using perm_j_type_ctx.
+Qed.
+
+Corollary perm_j_type_ctx_1 : forall Δ Γ1 Γ2 x τ2 t τ1,
+    (Δ ; (Γ1 ++ x ~ τ2) ++ Γ2 ⊢ t : τ1) <->
+    (Δ ; (Γ1 ++ Γ2) ++ x ~ τ2 ⊢ t : τ1).
+Proof.
+  intros. apply perm_j_type_ctx_iff.
+  apply permutation_fact.
+Qed.
+
+(** *** Weakening *)
+(******************************************************************************)
+Theorem weak_j_type_ctx : forall Δ Γ1 Γ2 t τ,
+    ok_type_ctx Δ Γ2 ->
+    disjoint Γ1 Γ2 ->
+    (Δ ; Γ1 ⊢ t : τ) ->
+    (Δ ; Γ1 ++ Γ2 ⊢ t : τ).
+Proof.
+  introv ok disj j.
+  (* save knowledge that Δ is uniq for [j_inst] case *)
+  pose proof (okΔ := j); apply j_kind_ctx_wf in okΔ.
+  induction j.
+  - apply j_var.
+    + assumption.
+    + now rewrite ok_type_ctx_app.
+    + autorewrite with tea_list. auto.
+  - apply j_abs with (L := L ∪ domset Γ2).
+    +  (* todo need better automation here *)
+      rename H0 into IH.
+      intros_cof IH; auto. rewrite <- perm_j_type_ctx_1.
+      apply IH; auto. autorewrite with tea_rw_disj. intuition fsetdec.
+  - apply j_app with (τ1 := τ1); auto.
+  - apply j_univ with (L := L ∪ domset Δ). intros_cof H0.
+    apply H0; auto.
+    + auto using ok_type_ctx_weak_r.
+    + rewrite ok_kind_ctx_app. autorewrite with tea_rw_disj.
+      splits; intuition (auto using ok_kind_ctx_one; fsetdec).
+  - apply j_inst.
+    + auto.
+    + apply IHj; auto.
+Qed.
+
+(** *** Substitution *)
+(******************************************************************************)
+Theorem subst_j_kind_ctx_1 : forall Δ x Γ t τ τ2,
+    ok_type Δ τ2 ->
+    (Δ ++ x ~ tt ; Γ ⊢ t : τ) ->
+    (Δ ; envmap (subst typ KType x τ2) Γ ⊢ subst term KType x τ2 t : subst typ KType x τ2 τ).
+Proof.
+  introv jτ jt. change_alist (Δ ++ x ~ tt ++ []) in jt.
+  change_alist (Δ ++ []) in jτ. change_alist (Δ ++ []).
+  auto using subst_j_kind_ctx.
+Qed.
+
+(** ** Properties in τ of <<(Δ ; Γ ⊢ t : τ>> *)
+(******************************************************************************)
+
+(** *** <<τ>> is always locally closed *)
+(******************************************************************************)
+Lemma j_lc_type : forall Δ Γ t τ,
+    (Δ ; Γ ⊢ t : τ) ->
+    locally_closed typ KType τ.
+Proof.
+  introv j. induction j.
+  - eapply ok_type_ctx_binds; eauto.
+  - cc. autorewrite with sysf_rw. (*split.
+    + eapply in_j_type_ctx2 in H. eapply ok_type_lc; eauto.
+    + auto.
+  - now autorewrite with sysf_rw in IHj1.
+  - cc. autorewrite with sysf_rw.
+    rewrite open_lc_gap_eq_var; eauto.
+  - autorewrite with sysf_rw in IHj.
+    rewrite <- open_lc_gap_eq_iff_1; eauto.
+    eapply ok_type_lc; eauto.
+*)
+Admitted.
+
+(** *** <<τ>> is always well-formed *)
+(******************************************************************************)
+Lemma j_ok_type : forall Δ Γ t τ,
+    (Δ ; Γ ⊢ t : τ) ->
+    ok_type Δ τ.
+Proof.
+  introv j. induction j.
+  - eauto using ok_type_ctx_binds.
+  - cc. rewrite ok_type_ar. split.
+    + eapply j_type_ctx2; eauto.
+    + auto.
+  - rewrite ok_type_ar in IHj1. tauto.
+  - rewrite ok_type_univ. rename H0 into IH.
+    pick fresh e for (L ∪ freeset typ KType τ).
+    specialize_cof IH e. destruct IH as [IHsc IHlc]. split.
+    + unfold ok_type, scoped in *.
+      enough (freeset typ KType τ ⊆ domset (Δ ++ e ~ tt)).
+      autorewrite with tea_rw_dom in H0. fsetdec.
+      rewrite (freeset_open_lower typ); eauto.
+    + rewrite (open_lc_gap_eq_iff typ); eauto.
+  (* now autorewrite with sysf_rw. *)
+      admit.
+  - rewrite ok_type_univ in IHj. destruct IHj.
+    unfold ok_type in *; split.
+    + unfold scoped in *.
+      rewrite (freeset_open_upper typ). fsetdec.
+    + unfold locally_closed.
+      rewrite (open_lc_gap_eq_iff typ) in H1;
+        eauto. tauto.
+Admitted.
+
+(** ** Properties in t of <<(Δ ; Γ ⊢ t : τ>> *)
+(******************************************************************************)
+
+(** *** <<t>> is always locally closed w.r.t. term variables *)
+(******************************************************************************)
+Lemma j_lc_KTerm_term : forall Δ Γ t τ,
+    (Δ ; Γ ⊢ t : τ) ->
+    locally_closed term KTerm t.
+Proof.
+  introv j. induction j.
+  - now simpl_F.
+  - cc. simpl_F.
+    rewrite open_lc_gap_eq_iff_1; eauto.
+    now simpl_F.
+  - now simpl_F.
+  - rename H0 into IH. cc.
+    autorewrite with sysf_rw.
+    rewrite (open_lc_gap_neq_var).
+    + exact IH.
+    + discriminate.
+  - simpl_F. intuition (auto using lc_term_type).
+Qed.
+
+(** *** <<t>> is always locally closed w.r.t. type variables *)
+(******************************************************************************)
+Lemma j_lc_KType_term : forall Δ Γ t τ,
+    (Δ ; Γ ⊢ t : τ) ->
+    locally_closed term KType t.
+Proof.
+  introv j. induction j.
+  - now simpl_F.
+  - cc. simpl_F. split.
+    + apply in_j_type_ctx2 in H. eapply ok_type_lc; eauto.
+    + rename Fr into fresh.
+      change (tm_var (Fr e)) with (mret SystemF KTerm (Fr e)) in H0.
+      rewrite <- (open_lc_gap_neq_var (H := I2) _ KTerm) in H0.
+      2:{ discriminate. }
+      auto.
+  - now simpl_F.
+  - rename H0 into IH. cc.
+    autorewrite with sysf_rw.
+    rewrite (open_lc_gap_eq_var).
+    + exact IH.
+    + auto.
+  - simpl_F. intuition (auto using lc_term_type).
+    eapply ok_type_lc; eauto.
+Qed.
+
+(** *** <<t>> is always well-scoped w.r.t. type variables *)
+(******************************************************************************)
+Lemma j_sc_KType_term : forall Δ Γ t τ,
+    (Δ ; Γ ⊢ t : τ) ->
+    scoped_env term KType t Δ.
+Proof.
+  introv j. induction j; unfold scoped_env, scoped in *.
+  - rewrite rw_freeset_KType_term12. fsetdec.
+  - simpl_F. cc.
+    assert (freeset typ KType τ1 ⊆ domset Δ).
+    { apply in_j_type_ctx2 in H. apply H. }
+    rewrite <- (freeset_open_lower) in H0.
+    fsetdec.
+  - simpl_F. fsetdec.
+  - simpl_F. cc. admit.
+  - simpl_F.
+    assert (freeset typ KType τ1 ⊆ domset Δ) by apply H.
+    fsetdec.
+Admitted.
+
+(** *** <<t>> is always well-scoped w.r.t. term variables *)
+(******************************************************************************)
+Lemma j_sc_KTerm_term : forall Δ Γ t τ,
+    (Δ ; Γ ⊢ t : τ) ->
+    scoped_env term KTerm t Γ.
+Proof.
+  introv j. induction j; unfold scoped_env, scoped in *.
+  - rewrite rw_freeset_KTerm_term12. admit.
+  - simpl_F. cc.
+    rewrite rw_freeset_KTerm_type.
+    rewrite <- (freeset_open_lower_eq) in H0.
+    admit.
+  - simpl_F. fsetdec.
+  - simpl_F. cc. admit.
+  - simpl_F.
+    rewrite rw_freeset_KTerm_type. fsetdec.
+Admitted.
+
+(** *** <<t>> is always well-formed *)
+(******************************************************************************)
+Lemma j_ok_tm_tm : forall Δ Γ t τ,
+    (Δ ; Γ ⊢ t : τ) ->
+    ok_term Δ Γ t.
+Proof.
+  intros. unfold ok_term.
+  intuition (eauto using j_sc_KTerm_term, j_sc_KType_term,
+             j_lc_KTerm_term, j_lc_KType_term).
+Qed.
+
+(** *** Substitution *)
+(******************************************************************************)
+Theorem subst_j_type_ctx : forall Δ Γ1 Γ2 x τ2 t u τ1,
+    (Δ ; Γ1 ++ x ~ τ2 ++ Γ2 ⊢ t : τ1) ->
+    (Δ ; Γ1 ++ Γ2 ⊢ u : τ2) ->
+    (Δ ; Γ1 ++ Γ2 ⊢ subst term KTerm x u t : τ1).
+Proof.
+  introv jt ju. remember (Γ1 ++ x ~ τ2 ++ Γ2) as Γ.
+  generalize dependent Γ2. induction jt; intros; subst.
+  - simpl_F. unfold subst_loc. compare values x and x0.
+    + enough (τ2 = τ) by congruence.
+      eapply in_uniq_mid_eq.
+      * inverts H0; eauto.
+      * assumption.
+    + constructor; eauto using ok_type_ctx_inv_mid, in_mid_neq.
+  - rename H0 into IH.
+    simpl_F. rewrite subst_KTerm_type.
+    apply j_abs with (L := L ∪ {{ x }} ∪ domset Γ1 ∪ domset Γ2).
+    intros_cof IH.
+    rewrite subst_open_eq in IH.
+    2:{ eapply j_lc_KTerm_term; eauto. }
+    rewrite subst_fresh in IH.
+    2:{ simpl_F. autorewrite with tea_list. fsetdec. }
+    simpl_alist in *. apply IH; auto.
+    change_alist ((Γ1 ++ Γ2) ++ e ~ τ1).
+    apply weak_j_type_ctx.
+    * apply ok_type_ctx_tm_one.
+      specialize_cof H e. eapply in_j_type_ctx2; eauto.
+    * autorewrite with tea_rw_disj in *. intuition fsetdec.
+    * assumption.
+  - simpl_F. eapply j_app; eauto.
+  - rename H0 into IH.
+    simpl_F. apply j_univ with (L := L).
+    intros_cof IH. rewrite subst_open_neq in IH.
+    2:{ discriminate. }
+    2:{ eapply j_ok_tm_tm; eauto. }
+    apply IH; eauto.
+    eapply weak_j_kind_ctx.
+    + admit.
+    + admit.
+    + admit.
+  - simpl_F. rewrite subst_KTerm_type. apply j_inst.
+    auto. apply IHjt. admit. auto.
+Admitted.
+
+Corollary subst_j_type_ctx_1 : forall Δ Γ x τ2 t u τ1,
+    (Δ ; Γ ++ x ~ τ2 ⊢ t : τ1) ->
+    (Δ ; Γ ⊢ u : τ2) ->
+    (Δ ; Γ ⊢ subst term KTerm x u t : τ1).
+Proof.
+  introv jt ju. change_alist (Γ ++ x ~ τ2 ++ []) in jt.
+  change_alist (Γ ++ []) in ju. change_alist (Γ ++ []).
+  eauto using subst_j_type_ctx.
+Qed.
+
+(** * Progress and preservation *)
+(******************************************************************************)
+Theorem preservation_theorem : preservation.
+Proof.
+  introv j. generalize dependent t'.
+  remember (@nil (atom * unit)) as Delta.
+  remember (@nil (atom * typ leaf)) as Gamma.
+  induction j; subst.
+  - inversion 1.
+  - inversion 1.
+  - inversion 1; subst.
+    + eauto using Judgment.
+    + eauto using Judgment.
+    + inverts j1. pick fresh e for (L ∪ freeset term KTerm t0).
+      rewrite (open_spec_eq term) with (x := e); [| fsetdec].
+      eapply subst_j_type_ctx_1; eauto.
+      apply H4. fsetdec.
+  - inversion 1.
+  - inversion 1; subst.
+    + eauto using Judgment.
+    + inverts j.
+      pick fresh e for (L ∪ freeset term KType t0 ∪ freeset typ KType τ2).
+      rewrite (open_spec_eq) with (x := e); [|fsetdec].
+      rewrite (open_spec_eq (F:=typ)) with (x := e); [|fsetdec].
+      change (@nil (atom * typ leaf))
+        with (subst (fun A : Type => alist typ A) KType e τ1 []).
+      apply subst_j_kind_ctx_1; auto.
+      apply H5. fsetdec.
+Qed.
+
+Theorem  progress_theorem : progress.
+Proof.
+  introv j. remember (@nil (atom * unit)) as Delta.
+  remember (@nil (atom * typ leaf)) as Gamma.
+  induction j; subst.
+  - inversion H1.
+  - left; auto using value.
+  - right. specialize (IHj1 ltac:(trivial) ltac:(trivial)).
+    specialize (IHj2 ltac:(trivial) ltac:(trivial)).
+    intuition.
+    + inverts H.
+      { eauto using red. }
+      { false. inverts j1. }
+    + inverts H.
+      { destruct_all_existentials.
+        eauto using red, value. }
+      { inverts j1. }
+    + destruct_all_existentials.
+      eauto using red.
+    + destruct_all_existentials.
+      eauto using red.
+  - left; auto using value.
+  - right. specialize (IHj ltac:(trivial) ltac:(trivial)).
+    intuition.
+    + inverts H0.
+      { inverts j. }
+      { eauto using red. }
+    + destruct_all_existentials.
+      eauto using red.
+Qed.
